implement SHA256 precompiled contract

Blanc.lean
@@ -2,100 +2,10 @@ import Lean.Data.Json
 import Lean.Data.Json.Parser
 import Lean.Data.HashSet
 import «Blanc».Weth
-
-def List.chunksCore {ξ} (m : Nat) : Nat → List ξ → List (List ξ)
-  | _, [] => [[]]
-  | 0, x :: xs =>
-    match chunksCore m m xs with
-    | [] => [[], [x]]
-    | ys :: yss => [] :: (x :: ys) :: yss
-  | n + 1, x :: xs =>
-    match chunksCore m n xs with
-    | [] => [[x]]
-    | ys :: yss => (x :: ys) :: yss
-
-def List.chunks {ξ} (m : Nat) : List ξ → List (List ξ) := List.chunksCore m (m + 1)
-
-def Bytes.toHexLine (bs : Bytes) : String :=
-  s!"hex\"{bs.toHex}\""
-
-def WethByteCode : String :=
-  List.foldr
-     (λ s0 s1 => s0 ++ "\n" ++ s1)
-     "" <| List.map Bytes.toHexLine
-        <| List.chunks 31 <| Option.getD weth.compile []
-
-def Strings.join : List String → String
-  | [] => ""
-  | s :: ss => s ++ "\n" ++ Strings.join ss
-
-def Hexit.toB4 : Char → Option B8
-  | '0' => some 0x00
-  | '1' => some 0x01
-  | '2' => some 0x02
-  | '3' => some 0x03
-  | '4' => some 0x04
-  | '5' => some 0x05
-  | '6' => some 0x06
-  | '7' => some 0x07
-  | '8' => some 0x08
-  | '9' => some 0x09
-  | 'a' => some 0x0A
-  | 'b' => some 0x0B
-  | 'c' => some 0x0C
-  | 'd' => some 0x0D
-  | 'e' => some 0x0E
-  | 'f' => some 0x0F
-  | 'A' => some 0x0A
-  | 'B' => some 0x0B
-  | 'C' => some 0x0C
-  | 'D' => some 0x0D
-  | 'E' => some 0x0E
-  | 'F' => some 0x0F
-  |  _  => none
-
-def B4L.toB8L : B8L → Option B8L
-  | [] => some []
-  | [_] => none
-  | x :: y :: xs =>
-    let xy := (x <<< 4) ||| y
-    (xy :: ·) <$> B4L.toB8L xs
-
-def Hex.toB8L (s : String) : Option B8L :=
-  s.data.mapM Hexit.toB4 >>= B4L.toB8L
-
-def Option.toIO {ξ} (o : Option ξ) (msg : String) : IO ξ := do
-  match o with
-  | none => throw (IO.Error.userError msg)
-  | some x => pure x
+import «Blanc».TestParse
 
 @[extern "ecrecover_flag"]
 opaque ecrecoverFlag : ByteArray → UInt8 → ByteArray → ByteArray
-
-def Bool.toByte : Bool → Byte
-  | true => Ox x0 x1
-  | false => Ox x0 x0
-
-structure Adr : Type where
-  (high : B32)
-  (mid : B64)
-  (low : B64)
-
-def Adr.toHex (a : Adr) : String :=
-  a.high.toHex ++ a.mid.toHex ++ a.low.toHex
-
-def B8L.toAdr : B8L → Option Adr
-  | x0 :: x1 :: x2 :: x3 ::
-    y0 :: y1 :: y2 :: y3 ::
-    y4 :: y5 :: y6 :: y7 ::
-    z0 :: z1 :: z2 :: z3 ::
-    z4 :: z5 :: z6 :: z7 :: _ =>
-    some ⟨
-      B8s.toB32 x0 x1 x2 x3,
-      B8s.toB64 y0 y1 y2 y3 y4 y5 y6 y7,
-      B8s.toB64 z0 z1 z2 z3 z4 z5 z6 z7,
-    ⟩
-  | _ => none
 
 def ecrecover (h : B256) (v : Bool) (r : B256) (s : B256) : Option Adr :=
   let rsa : ByteArray := ⟨Array.mk (r.toB8L ++ s.toB8L)⟩
@@ -108,547 +18,13 @@ def ecrecover (h : B256) (v : Bool) (r : B256) (s : B256) : Option Adr :=
     then none
     else B8L.toAdr pa
 
-def readJsonFile (filename : System.FilePath) : IO Lean.Json := do
-  let contents ← IO.FS.readFile filename
-  match Lean.Json.parse contents with
-  | .ok json => pure json
-  | .error err => throw (IO.userError err)
-
-mutual
-  partial def StringJsons.toStrings : List ((_ : String) × Lean.Json) → List String
-    | [] => []
-    | sj :: sjs =>
-      (sj.fst :: Lean.Json.toStrings sj.snd) ++ StringJsons.toStrings sjs
-
-  partial def Lean.Jsons.toStrings : List Lean.Json → List String
-    | [] => []
-    | j :: js => Lean.Json.toStrings j ++ Lean.Jsons.toStrings js
-
-  partial def Lean.Json.toStrings : Lean.Json → List String
-    | .null => ["null"]
-    | .bool b => [s!"bool : {b}"]
-    | .num n => [s!"num : {n}"]
-    | .str s => [s!"str : {s}"]
-    | .arr js =>
-      "arr :" :: (Lean.Jsons.toStrings js.toList).map ("  " ++ ·)
-    | .obj m => do
-      let kvs := m.toArray.toList
-      "obj : " :: (StringJsons.toStrings kvs).map ("  " ++ ·)
-end
-
-def Lean.Json.toString (j : Lean.Json) : String := Strings.join j.toStrings
-
-def Adr.ordering : Adr → Adr → Ordering
-  | ⟨xh, xm, xl⟩, ⟨yh, ym, yl⟩ =>
-    match compare xh yh with
-    | .eq =>
-      match compare xm ym with
-      | .eq => compare xl yl
-      | o => o
-    | o => o
-
-instance : Ord Adr := ⟨Adr.ordering⟩
-
-def List.compare {ξ : Type u} [Ord ξ] : List ξ → List ξ → Ordering
-  | [], [] => .eq
-  | [], _ :: _ => .lt
-  | _ :: _, [] => .gt
-  | x :: xs, y :: ys =>
-    match Ord.compare x y with
-    | .eq => List.compare xs ys
-    | o => o
-
-def B128.compare : B128 → B128 → Ordering
-  | ⟨x, y⟩, ⟨x', y'⟩ =>
-    match Ord.compare x x' with
-    | .eq => Ord.compare y y'
-    | o => o
-
-instance : Ord B128 := ⟨B128.compare⟩
-
-def B256.compare : B256 → B256 → Ordering
-  | ⟨x, y⟩, ⟨x', y'⟩ =>
-    match Ord.compare x x' with
-    | .eq => Ord.compare y y'
-    | o => o
-
-instance {ξ : Type u} [Ord ξ] : Ord (List ξ) := ⟨List.compare⟩
-instance : Ord B256 := ⟨B256.compare⟩
-
-def B8.compareLows (x y : B8) : Ordering :=
-  Ord.compare x.lows y.lows
-
 abbrev NTB := Lean.RBMap (List B8) (List B8) (@List.compare _ ⟨B8.compareLows⟩)
-
-abbrev Stor := Lean.RBMap B256 B256 compare
-
-structure EnvData where
-  (baseFee : B256)
-  (coinbase : Adr)
-  (prevRandao : B256)
-  (blockGasLimit : B256)
-  (timestamp : B256)
-  (number : B256)
-
-structure PreData where
-  (addr : Adr)
-  (nonce : B8L)
-  (bal : B8L)
-  (stor : Stor)
-  (code : B8L)
-
-structure PostData where
-  (hash : B256)
-  (dataIdx : Nat)
-  (gasIdx : Nat)
-  (valueIdx : Nat)
-  (logs : B256)
-  (txdata : B8L)
-
-structure TransactionData : Type where
-  (data : List B8L)
-  (gasLimit : List B256)
-  (gasPrice : B256)
-  (nonce : B256)
-  (secretKey : B256)
-  (sender : Adr)
-  (receiver : Adr)
-  (value : List B256)
-
-structure TestData where
-  (info : Lean.Json)
-  (env  : EnvData)
-  (pre  : List PreData)
-  (post : String × List PostData)
-  (tx   : TransactionData)
-
-structure Acct where
-  (nonce : B256)
-  (bal : B256)
-  (stor : Stor)
-  (code : ByteArray)
-
-abbrev Wor : Type := Lean.RBMap Adr Acct compare
-
-structure Test where
-  (baseFee : B256)
-  (coinbase : Adr)
-  (prevRandao : B256)
-  (blockGasLimit : B256)
-  (number : B256)
-  (timestamp : B256)
-
-  (world  : Wor)
-  (txdata : B8L)
-
-  (nonce : B256)
-  (gasPrice : B256)
-  (gasLimit : B256)
-  (sender : Adr)
-  (receiver : Adr)
-  (value : B256)
-  (calldata : B8L)
-
-  (hash : B256) -- ?
-  (logs : B256) -- keccak hash of (RLP-encoded) log items
-  (secret : B256)
-
-def pad : String → String
-  | s => "  " ++ s
-
-def padMid : String -> String
-  | s => "│ " ++ s
-
-def padsMid : List String → List String
-  | [] => []
-  | s :: ss => ("├─" ++ s) :: ss.map padMid
-
-def padsEnd : List String → List String
-  | [] => []
-  | s :: ss => ("└─" ++ s) :: ss.map pad
-
-def padss : List (List String) -> List String
-  | [] => []
-  | [ss] => padsEnd ss
-  | ss :: sss => padsMid ss ++ padss sss
-
-def fork (s : String) : List (List String) → List String
-  | [[s']] => [s ++ "──" ++ s']
-  | sss => s :: padss sss
-
-def encloseStrings : List String → List String
-  | [] => ["[]"]
-  | [s] => ["[" ++ s ++ "]"]
-  | ss => "┌─" :: ss.map padMid ++ ["└─"]
-
-def listToStrings {ξ} (f : ξ -> List String) (xs : List ξ) : List String :=
-  encloseStrings (xs.map f).flatten
-
-def longB8LToStrings (hd : String) (bs : B8L) : List String :=
-  match List.chunks 31 bs with
-  | [] => [hd]
-  | [bs'] => [s!"{hd} : {B8L.toHex bs'}"]
-  | bss => s!"{hd} :" :: bss.map (λ bs' => pad (B8L.toHex bs'))
-
-def txdataToStrings (tx : B8L) : List String :=
-  match List.chunks 31 tx with
-  | [] => ["txdata :"]
-  | [bs] => [s!"txdata : {B8L.toHex bs}"]
-  | bss => "txdata :" :: bss.map (λ bs => pad (B8L.toHex bs))
-
-def Stor.toStrings (s : Stor) : List String :=
-  let kvs := s.toArray.toList
-  let kvToStrings : B256 × B256 → List String :=
-    λ nb => [s!"{B256.toHex nb.fst} : {B256.toHex nb.snd}"]
-  fork "stor" (kvs.map kvToStrings)
-
-def Acct.toStrings (s : String) (a : Acct) : List String :=
-  fork s [
-    [s!"nonce : 0x{a.nonce.toHex}"],
-    [s!"bal : 0x{a.bal.toHex}"],
-    a.stor.toStrings,
-    longB8LToStrings "code" a.code.toList
-  ]
-
-def postAcct.toStrings (p : PostData) : List String :=
-  fork "Post Acct" [
-    [s!"hash : {p.hash.toHex}"],
-    [s!"data index : {p.dataIdx}"],
-    [s!"gas index : {p.gasIdx}"],
-    [s!"value index : {p.valueIdx}"],
-    [s!"logs : {B256.toHex p.logs}"],
-    txdataToStrings p.txdata
-  ]
-
-def Lean.RBMap.toStrings {α β cmp} (m : Lean.RBMap α β cmp)
-  (fmt : α × β → List String): List String :=
-  let kvs := m.toArray.toList
-  fork "map" (kvs.map fmt)
-
-def Wor.toStrings (w : Wor) : List String :=
-  let kvs := w.toArray.toList
-  let kvToStrings : Adr × Acct → List String :=
-    fun x => Acct.toStrings x.fst.toHex x.snd
-  fork "world" (kvs.map kvToStrings)
-
-def B4L.toHex : B8L → String
-  | [] => ""
-  | [b] => ⟨[b.toHexit]⟩
-  | b :: bs => ⟨[b.toHexit] ++ (toHex bs).data⟩
 
 def NTB.toStrings (s : NTB) : List String :=
   let kvs := s.toArray.toList
   let kvToStrings : B8L × B8L → List String :=
     λ nb => [s!"{B4L.toHex (nb.fst.map B8.lows)} : {nb.snd.toHex}"]
   fork "NTB" (kvs.map kvToStrings)
-
-def preAcct.toStrings (p : PreData) : List String :=
-  fork "Pre Acct" [
-    [s!"address : {p.addr.toHex}"],
-    [s!"nonce : {B8L.toHex p.nonce}"],
-    [s!"balance : {B8L.toHex p.bal}"],
-    p.stor.toStrings,
-    [s!"code : {B8L.toHex p.code}"]
-  ]
-
-def postToStrings : (String × List PostData) → List String
-  | ⟨s, ps⟩ => fork "Post" [[s], listToStrings postAcct.toStrings ps]
-
-def EnvData.toStrings (e : EnvData) : List String :=
-  fork "env" [
-    [s!"coinbase : {e.coinbase.toHex}"],
-  ]
-
-def preToStrings (l : List PreData) : List String :=
-  fork "pre" [listToStrings preAcct.toStrings l]
-
-def TransactionData.toStrings (tx : TransactionData) : List String :=
-  fork "transaction" [
-    fork "data" [listToStrings (λ x => [B8L.toHex x]) tx.data],
-    fork "gasLimit" [listToStrings (λ x => [x.toHex]) tx.gasLimit],
-    [s!"gasPrice : {tx.gasPrice.toHex}"],
-    [s!"nonce :     {tx.nonce.toHex}"],
-    [s!"secretKey : {tx.secretKey.toHex}"],
-    [s!"sender : {tx.sender.toHex}"],
-    [s!"to : {tx.receiver.toHex}"],
-    fork "value" [listToStrings (λ x => [x.toHex]) tx.value]
-  ]
-
-def Test.toStrings (t : Test) : List String :=
-  fork "VM Test" [
-    [s!"coinbase : {t.coinbase.toHex}"],
-    t.world.toStrings,
-    txdataToStrings t.txdata,
-    [s!"nonce : 0x{t.nonce.toHex}"],
-    [s!"gas price : 0x{t.gasPrice.toHex}"],
-    [s!"gas limit : 0x{t.gasLimit.toHex}"],
-    [s!"sender : 0x{t.sender.toHex}"],
-    [s!"receiver : 0x{t.receiver.toHex}"],
-    [s!"value : 0x{t.value.toHex}"],
-    longB8LToStrings "calldata" t.calldata,
-    [s!"hash : 0x{t.hash.toHex}"],
-    [s!"logs : 0x{t.logs.toHex}"],
-    [s!"secret : 0x{t.secret.toHex}"]
-  ]
-
-def TestData.toStrings (t : TestData) : List String :=
-  fork "VM Test" [
-    ["info ..."],--t.info.toStrings,
-    EnvData.toStrings t.env,
-    preToStrings t.pre,
-    postToStrings t.post,
-    t.tx.toStrings
-  ]
-
-def TestData.toString (t : TestData) : String := Strings.join t.toStrings
-def Test.toString (t : Test) : String := Strings.join t.toStrings
-
-def IO.throw {ξ} (s : String) : IO ξ := MonadExcept.throw <| IO.Error.userError s
-
-def Lean.Json.fromArr : Lean.Json → IO (List Json)
-  | .arr a => return a.toList
-  | _ => IO.throw "not an array"
-
-def Lean.Json.fromObj : Lean.Json → IO (RBNode String (λ _ => Json))
-  | .obj r => return r
-  | _ => IO.throw "not an object"
-
-def Lean.Json.fromStr : Lean.Json → IO String
-  | .str s => return s
-  | _ => IO.throw "not a string"
-
-def Lean.Json.fromNum : Lean.Json → IO JsonNumber
-  | .num n => return n
-  | _ => IO.throw "not a string"
-
-def Lean.JsonNumber.toNat : JsonNumber → IO Nat
-  | ⟨.ofNat x, 0⟩ => return x
-  | ⟨.negSucc _, _⟩ => IO.throw "negative mantissa"
-  | ⟨_, e + 1⟩ => IO.throw s!"nonzero exponent : {e + 1}"
-
-def Lean.Json.fromSingleton : Lean.Json → IO (String × Lean.Json)
-  | .obj (.node _ .leaf k v .leaf) => return ⟨k, v⟩
-  | _ => IO.throw "not a singleton"
-
-def Hex.from0x : String → IO String
-  | ⟨'0' :: 'x' :: s⟩ => return ⟨s⟩
-  | _ => IO.throw "prefix not 0x"
-
-def B8s.toB128
-  (x0 x1 x2 x3 x4 x5 x6 x7 y0 y1 y2 y3 y4 y5 y6 y7 : B8) : B128 :=
-  ⟨ B8s.toB64 x0 x1 x2 x3 x4 x5 x6 x7,
-    B8s.toB64 y0 y1 y2 y3 y4 y5 y6 y7 ⟩
-
-def B8s.toB256
-  ( x0 x1 x2 x3 x4 x5 x6 x7 x8 x9 xA xB xC xD xE xF
-    y0 y1 y2 y3 y4 y5 y6 y7 y8 y9 yA yB yC yD yE yF : B8 ) : B256 :=
-  ⟨ B8s.toB128 x0 x1 x2 x3 x4 x5 x6 x7 x8 x9 xA xB xC xD xE xF,
-    B8s.toB128 y0 y1 y2 y3 y4 y5 y6 y7 y8 y9 yA yB yC yD yE yF ⟩
-
-def B8L.toB128Diff : B8L → Option (B128 × B8L)
-  | x0 :: x1 :: x2 :: x3 ::
-    x4 :: x5 :: x6 :: x7 ::
-    y0 :: y1 :: y2 :: y3 ::
-    y4 :: y5 :: y6 :: y7 :: xs =>
-    some ⟨
-        ⟨ B8s.toB64 x0 x1 x2 x3 x4 x5 x6 x7,
-          B8s.toB64 y0 y1 y2 y3 y4 y5 y6 y7 ⟩,
-        xs
-      ⟩
-  | _ => none
-
-def List.ekatD {ξ : Type u} (n : Nat) (xs : List ξ) (x : ξ) : List ξ :=
-  (xs.reverse.takeD n x).reverse
-
-lemma List.length_ekatD {ξ : Type u} (n : Nat) (xs : List ξ) (x : ξ) :
-    (List.ekatD n xs x).length = n := by
-  apply Eq.trans (List.length_reverse _)
-  apply Eq.trans (List.takeD_length _ _ _) rfl
-
-def B8L.toB256? (xs : B8L) : Option B256 := do
-  let ⟨h, xs'⟩ ← xs.toB128Diff
-  let ⟨l, []⟩ ← xs'.toB128Diff | none
-  some ⟨h, l⟩
-
-def Hex.toB256? (hx : String) : Option B256 := do
-  Hex.toB8L hx >>= B8L.toB256?
-
-def B8V.toB128 : Vec B8 16 → B128
-  | ⟨ [ b0, b1, b2, b3, b4, b5, b6, b7,
-        b8, b9, bA, bB, bC, bD, bE, bF ], _ ⟩ =>
-    ⟨ B8s.toB64 b0 b1 b2 b3 b4 b5 b6 b7,
-      B8s.toB64 b8 b9 bA bB bC bD bE bF ⟩
-
-def B8V.toB256 (xs : Vec B8 32) : B256 :=
-  let h : Vec B8 16 := xs.take 16
-  let l : Vec B8 16 := xs.drop 16
-  ⟨B8V.toB128 h, B8V.toB128 l⟩
-
-def B8L.pack (xs : B8L) (n : Nat) : B8L := List.ekatD n xs 0
-
-def B8L.toB8V (xs : B8L) (n : Nat) : Vec B8 n :=
-  ⟨xs.pack n, List.length_ekatD _ _ _⟩
-
-def B8L.toB256P (xs : B8L) : B256 := B8V.toB256 (xs.toB8V 32)
-
-def Lean.Json.toPostData : Json → IO PostData
-  | .obj r => do
-    let hsx ← (r.find compare "hash").toIO "cannot retrieve hash bytes" >>= fromStr >>= Hex.from0x
-    let hs ← (Hex.toB256? hsx).toIO "cannot convert hash bytes to word"
-    let lgx ← (r.find compare "logs").toIO "cannot get logs bytes" >>= fromStr >>= Hex.from0x
-    let lg ← (Hex.toB256? lgx).toIO "cannot convert logs bytes to word"
-    let txx ← (r.find compare "txbytes").toIO "cannot get tx bytes" >>= fromStr >>= Hex.from0x
-    let tx ← (Hex.toB8L txx).toIO "cannot convert tx bytes to word"
-    let dgv ← (r.find compare "indexes").toIO "cannot get indexes" >>= Json.fromObj
-    let d ← (dgv.find compare "data").toIO "cannot get data" >>= Json.fromNum >>= JsonNumber.toNat
-    let g ← (dgv.find compare "gas").toIO "cannot get gas" >>= Json.fromNum >>= JsonNumber.toNat
-    let v ← (dgv.find compare "value").toIO "cannot get value" >>= Json.fromNum >>= JsonNumber.toNat
-    return ⟨hs, d, g, v, lg, tx⟩
-  | _ => IO.throw "Json-to-PostData failed"
-
-def Lean.Json.toB8L (j : Json) : IO B8L := do
-  let x ← fromStr j >>= Hex.from0x
-  (Hex.toB8L x).toIO ""
-
-def Hex.toAdr (hx : String) : Option Adr := Hex.toB8L hx >>= B8L.toAdr
-
-def Lean.Json.toAdr (j : Json) : IO Adr := do
-  let x ← fromStr j >>= Hex.from0x
-  (Hex.toAdr x).toIO ""
-
-def Lean.Json.toB256? (j : Json) : IO B256 := do
-  let x ← fromStr j >>= Hex.from0x
-  (Hex.toB256? x).toIO ""
-
-def Lean.Json.toB256P (j : Json) : IO B256 := do
-  let x ← fromStr j >>= Hex.from0x
-  let xs ← (Hex.toB8L x).toIO ""
-  return (B8L.toB256P xs)
-
-def helper (xy :(_ : String) × Lean.Json) : IO (B256 × B256) := do
-  let x ← Hex.from0x xy.fst
-  let bs ← (Hex.toB8L x).toIO ""
-  let bs' ← xy.snd.toB8L
-  return ⟨bs.toB256P, bs'.toB256P⟩
-
-def Lean.Json.toPreData (sj : (_ : String) × Json) : IO PreData := do
-  let ax ← Hex.from0x sj.fst
-  let a ← (Hex.toAdr ax).toIO ""
-  let r ← sj.snd.fromObj
-  let b ← (r.find Ord.compare "balance").toIO "" >>= toB8L
-  let c ← (r.find Ord.compare "code").toIO "" >>= toB8L
-  let n ← (r.find Ord.compare "nonce").toIO "" >>= toB8L
-  let l ← (r.find Ord.compare "storage").toIO "" >>= fromObj
-  let s ← mapM helper l.toArray.toList
-  return ⟨a, n, b, Lean.RBMap.fromList s _, c⟩
-
-def Lean.Json.toEnvData (j : Lean.Json) : IO EnvData := do
-  let r ← j.fromObj
-  let bfj ← (r.find compare "currentBaseFee").toIO "No basefee"
-  let cbj ← (r.find compare "currentCoinbase").toIO "No coinbase"
-  let prj ← (r.find compare "currentRandom").toIO "No random"
-  let glj ← (r.find compare "currentGasLimit").toIO "No gas limit"
-  let tsj ← (r.find compare "currentTimestamp").toIO "No timestamp"
-  let nj  ← (r.find compare "currentNumber").toIO "No number"
-  let bf ← bfj.toB256P
-  let cb ← cbj.toAdr
-  let pr ← prj.toB256?
-  let gl ← glj.toB256P
-  let ts ← tsj.toB256P
-  let n  ← nj.toB256P
-  return {
-    baseFee := bf
-    coinbase := cb
-    prevRandao := pr
-    blockGasLimit := gl
-    timestamp := ts
-    number := n
-  }
-
-def Lean.Json.toPreDatas (j : Lean.Json) : IO (List PreData) := do
-  let r ← j.fromObj
-  let kvs := r.toArray.toList
-  mapM Lean.Json.toPreData kvs
-
-def Lean.Json.toPost (j : Lean.Json) : IO (String × List PostData) := do
-  let ⟨k, j'⟩ ← j.fromSingleton
-  let l ← j'.fromArr
-  let js ← mapM Lean.Json.toPostData l
-  return ⟨k, js⟩
-
-def Lean.Json.toTransactionData (j : Lean.Json) : IO TransactionData := do
-  let r ← j.fromObj
-  let ds ← (r.find Ord.compare "data").toIO "" >>= fromArr >>= mapM toB8L
-  let gls ← (r.find Ord.compare "gasLimit").toIO "" >>= fromArr >>= mapM toB256P
-  let gp ← ((r.find Ord.compare "gasPrice").toIO "" >>= toB256P)
-  let n ← ((r.find Ord.compare "nonce").toIO "" >>= toB256P)
-  let sk ← (r.find Ord.compare "secretKey").toIO "" >>= toB256?
-  let sd ← (r.find Ord.compare "sender").toIO "" >>= toAdr
-  let rc ← (r.find Ord.compare "to").toIO "" >>= toAdr
-  let vs ← (r.find Ord.compare "value").toIO "" >>= fromArr >>= mapM toB256P
-  return ⟨ds, gls, gp, n, sk, sd, rc, vs⟩
-
-def Lean.Json.toTestData (j : Lean.Json) : IO TestData := do
-  let (_, .obj r) ← j.fromSingleton | IO.throw "not singleton object"
-  let info ← (r.find compare "_info").toIO ""
-  let env ←  (r.find compare "env").toIO "" >>= Lean.Json.toEnvData
-  let pre ←  (r.find compare "pre").toIO "" >>= Lean.Json.toPreDatas
-  let post ← (r.find compare "post").toIO "" >>= Lean.Json.toPost
-  let tx ←   (r.find compare "transaction").toIO "" >>= Lean.Json.toTransactionData
-  return ⟨info, env, pre, post, tx⟩
-
-
-def TestData.world (td : TestData) : Option Wor :=
-  let aux : PreData → Option (Adr × Acct) :=
-    fun pd => do
-      some  ⟨
-        pd.addr,
-        {
-          nonce := pd.nonce.toB256P
-          bal := pd.bal.toB256P
-          stor := pd.stor
-          code := ByteArray.mk <| Array.mk pd.code
-        }
-    ⟩
-  do let l ← List.mapM aux td.pre
-     some <| Lean.RBMap.fromList l _
-
-def getTest (td : TestData) (p : PostData) : IO Test := do
-  let cd ← (List.get? td.tx.data p.dataIdx).toIO ""
-  let gl ← (List.get? td.tx.gasLimit p.gasIdx).toIO ""
-  let vl ← (List.get? td.tx.value p.valueIdx).toIO ""
-  let w ← td.world.toIO ""
-  return {
-    baseFee := td.env.baseFee
-    coinbase := td.env.coinbase
-    prevRandao := td.env.prevRandao
-    blockGasLimit := td.env.blockGasLimit
-    number := td.env.number
-    timestamp := td.env.timestamp
-    world := w
-    txdata := p.txdata
-    calldata := cd
-    gasLimit := gl
-    gasPrice := td.tx.gasPrice
-    nonce := td.tx.nonce
-    secret := td.tx.secretKey
-    sender := td.tx.sender
-    receiver := td.tx.receiver
-    value := vl
-    hash := p.hash
-    logs := p.logs
-  }
-
-def getTests (t : TestData) : IO (List Test) := do
-  have ps := t.post.snd
-  mapM (getTest t) ps
-
-def Lean.RBMap.fromSingleton {ξ υ f} (m : RBMap ξ υ f) : Option (ξ × υ) :=
-  match m.toList with
-  | [kv] => some kv
-  | _ => none
-
-def Lean.RBMap.singleton {ξ υ f} (x : ξ) (y : υ) : RBMap ξ υ f := RBMap.empty.insert x y
 
 def hpAux : B8L → (Option B8 × B8L)
   | [] => ⟨none, []⟩
@@ -773,16 +149,9 @@ def trie (j : NTB) : B256 :=
   let bs := (collapse j).encode
   bs.keccak
 
-def B256.toRLP (w : B256) : RLP' := .b8s w.toB8L
-def B16.toB8L (x : B16) : List B8 := [x.highs, x.lows]
-def B32.toB8L (x : B32) : List B8 := x.highs.toB8L ++ x.lows.toB8L
-def B8.toB4s (x : B8) : List B8 := [x.highs, x.lows]
-def B16.toB4s (x : B16) : List B8 := x.highs.toB4s ++ x.lows.toB4s
-def B32.toB4s (x : B32) : List B8 := x.highs.toB4s ++ x.lows.toB4s
-def B64.toB4s (x : B64) : List B8 := x.highs.toB4s ++ x.lows.toB4s
-def B128.toB4s (x : B128) : List B8 := x.1.toB4s ++ x.2.toB4s
-def B256.toB4s (x : B256) : List B8 := x.1.toB4s ++ x.2.toB4s
+
 def B256.keccak (x : B256) : B256 := B8L.keccak <| x.toB8L
+def B256.toRLP (w : B256) : RLP' := .b8s w.toB8L
 
 def B8L.sig (bs : B8L) : B8L := List.dropWhile (· = 0) bs
 
@@ -805,22 +174,8 @@ def Acct.toVal (a : Acct) (w : B256) : B8L :=
     .b8s a.nonce.toB8L.sig,
     .b8s a.bal.toB8L.sig,
     B256.toRLP w,
-    B256.toRLP <| B8L.keccak (a.code.toList)
+    B256.toRLP <| ByteArray.keccak 0 a.code.size a.code
   ]
-
-def compareRLP : RLP → RLP' → Option Unit
-  | .bytes xs, .b8s ys =>
-    if (xs = List.map B8.toByte ys)
-    then some ()
-    else none
-  | .list [], .list [] => some ()
-  | .list (x :: xs), .list (y :: ys) => do
-    (compareRLP x y)
-    compareRLP (.list xs) (.list ys)
-  | _, _ => none
-
-def Adr.toB8L (a : Adr) : B8L :=
-  a.high.toB8L ++ a.mid.toB8L ++ a.low.toB8L
 
 def toKeyVal (pr : Adr × Acct) : B8L × B8L :=
   let ad := pr.fst
@@ -840,13 +195,32 @@ def toKeyVal (pr : Adr × Acct) : B8L × B8L :=
 
 -- values --
 
-def G_txcreate : Nat := 32000
-def G_accesslistaddress : Nat := 2400
-def G_accessliststorage : Nat := 1900
-def G_initcodeword : Nat := 2
+def gHigh : Nat := 10
+def gJumpdest : Nat := 1
+def gTxcreate : Nat := 32000
+def gAccesslistaddress : Nat := 2400
+def gAccessliststorage : Nat := 1900
+def gInitcodeword : Nat := 2
+def gBase : Nat := 2
+def gCopy : Nat := 3
+def gMemory : Nat := 3
+def gKeccak256 : Nat := 30
+def gKeccak256Word : Nat := 6
+def cMem (a : Nat) := gMemory * a + ((a ^ 2) / 512)
+-- def gZero : Nat := 0
+def gVerylow : Nat := 3
+def gLow : Nat := 5
+def gMid : Nat := 8
+def gExp : Nat := 10
+def gExpbyte : Nat := 50
+def gColdSLoad : Nat := 2100
+def gSSet : Nat := 20000
+def gSReset : Nat := 2900
+def rSClear : Nat := 4800
+def gTransaction : Nat := 21000
 
 def initCodeCost (cd : B8L) : Nat :=
-  G_initcodeword * ((cd.length / 32) + if 32 ∣ cd.length then 0 else 1)
+  gInitcodeword * ((cd.length / 32) + if 32 ∣ cd.length then 0 else 1)
 
 instance {a b : Adr} : Decidable (a = b) := by
   cases a; cases b; simp; apply instDecidableAnd
@@ -891,7 +265,6 @@ def Var.toAcs (υ : Var) : Acs :=
     tchd := υ.tchd
   }
 
-def ceilDiv (m n : Nat) := m / n + if m % n = 0 then 0 else 1
 
 -- μ_i : no need to make it a separate field of Machine,
 -- when it is completely determined by Machine.mem
@@ -907,16 +280,18 @@ structure Block where
   (chainId : B256) -- β
 
 structure Con where
-  (cta : Adr) -- contract address (YP : a)
-  (oga : Adr) -- origin address (YP : o)
-  (gpr : B256) -- gas price (YP : p)
-  (cld : B8L) -- calldata (YP : d)
-  (cla : Adr) -- caller Addr (YP : s)
-  (clv : B256) -- callvalue (YP : v)
-  (code : ByteArray) -- contract code  (YP : b)
   (blk : Block) -- block (YP : H)
-  (exd : Nat) -- execution depth (YP : e)
-  (wup : Bool) -- World-State update permission (YP : w)
+  (wor0 : Wor)
+
+  (cta : Adr) -- contract address (YP : I_a)
+  (oga : Adr) -- origin address (YP : I_o)
+  (gpr : B256) -- gas price (YP : I_p)
+  (cld : B8L) -- calldata (YP : I_d)
+  (cla : Adr) -- caller Addr (YP : I_s)
+  (clv : B256) -- callvalue (YP : I_v)
+  (code : ByteArray) -- contract code  (YP : I_b)
+  (exd : Nat) -- execution depth (YP : I_e)
+  (wup : Bool) -- World-State update permission (YP : I_w)
 
 -- YP says that this type should also have a field for
 -- execution environment, but it was omitted since the
@@ -937,11 +312,6 @@ lemma List.length_takeD {ξ : Type u} (n : Nat) (xs : List ξ) (x : ξ) :
   induction n with
   | zero => rfl
   | succ n ih => simp [takeD]
-
-def Nat.decrement : Nat → Nat → Option Nat
-  | m, 0 => some m
-  | 0, _ + 1 => none
-  | m + 1, n + 1 => Nat.decrement m n
 
 def Jinst.toString : Jinst → String
   | .jump => "JUMP"
@@ -979,10 +349,6 @@ def noPushBefore (cd : Array B8) : Nat → Nat → Bool
            then false
            else noPushBefore cd k m
 
-def Jinst.toB8 : Jinst → B8
-  | jump => 0x56     -- 0x56 / 1 / 0 / Unconditional jump.
-  | jumpi => 0x57    -- 0x57 / 2 / 0 / Conditional jump.
-  | jumpdest => 0x5B -- 0x5b / 0 / 0 / Mark a valid jump destination.
 
 def jumpable' (cd : ByteArray) (k : Nat) : Bool :=
   if cd.get! k = (Jinst.toB8 .jumpdest)
@@ -993,156 +359,6 @@ def jumpable (cd : Array B8) (k : Nat) : Bool :=
   if cd.get? k = some (Jinst.toB8 .jumpdest)
   then noPushBefore cd k 32
   else false
-
-def ByteArray.sliceD (xs : ByteArray) : Nat → Nat → B8 → B8L
-  | _, 0, _ => []
-  | m, n + 1, d => --xs.getD m d :: Array.sliceD xs (m + 1) n d
-    if m < xs.size
-    then xs.get! m :: ByteArray.sliceD xs (m + 1) n d
-    else List.replicate (n + 1) d
-
-lemma ByteArray.length_sliceD {xs : ByteArray} {m n x} :
-    (ByteArray.sliceD xs m n x).length = n := by
-  induction n generalizing m with
-  | zero => simp [sliceD]
-  | succ n ih =>
-    simp [sliceD]
-    by_cases h : m < xs.size
-    · rw [if_pos h]; simp [List.length]; apply ih
-    · rw [if_neg h]; apply List.length_replicate
-
-def Array.sliceD {ξ : Type u} (xs : Array ξ) : Nat → Nat → ξ → List ξ
-  | _, 0, _ => []
-  | m, n + 1, d => xs.getD m d :: Array.sliceD xs (m + 1) n d
-
-lemma Array.length_sliceD {ξ} {xs : Array ξ} {m n x} :
-    (Array.sliceD xs m n x).length = n := by
-  induction n generalizing m with
-  | zero => simp [sliceD]
-  | succ n ih => simp [sliceD, List.length, ih]
-
-def B8.toRinst : B8 → Option Rinst
-  | 0x01 => some .add -- 0x01 / 2 / 1 / addition operation.
-  | 0x02 => some .mul -- 0x02 / 2 / 1 / multiplication operation.
-  | 0x03 => some .sub -- 0x03 / 2 / 1 / subtraction operation.
-  | 0x04 => some .div -- 0x04 / 2 / 1 / integer division operation.
-  | 0x05 => some .sdiv -- 0x05 / 2 / 1 / signed integer division operation.
-  | 0x06 => some .mod -- 0x06 / 2 / 1 / modulo operation.
-  | 0x07 => some .smod -- 0x07 / 2 / 1 / signed modulo operation.
-  | 0x08 => some .addmod -- 0x08 / 3 / 1 / modulo addition operation.
-  | 0x09 => some .mulmod -- 0x09 / 3 / 1 / modulo multiplication operation.
-  | 0x0a => some .exp -- 0x0a / 2 / 1 / exponentiation operation.
-  | 0x0b => some .signextend -- 0x0b / 2 / 1 / sign extend operation.
-  | 0x10 => some .lt -- 0x10 / 2 / 1 / less-than comparison.
-  | 0x11 => some .gt -- 0x11 / 2 / 1 / greater-than comparison.
-  | 0x12 => some .slt -- 0x12 / 2 / 1 / signed less-than comparison.
-  | 0x13 => some .sgt -- 0x13 / 2 / 1 / signed greater-than comparison.
-  | 0x14 => some .eq -- 0x14 / 2 / 1 / equality comparison.
-  | 0x15 => some .iszero -- 0x15 / 1 / 1 / tests if the input is zero.
-  | 0x16 => some .and -- 0x16 / 2 / 1 / bitwise and operation.
-  | 0x17 => some .or -- 0x17 / 2 / 1 / bitwise or operation.
-  | 0x18 => some .xor -- 0x18 / 2 / 1 / bitwise xor operation.
-  | 0x19 => some .not -- 0x19 / 1 / 1 / bitwise not operation.
-  | 0x1a => some .byte -- 0x1a / 2 / 1 / retrieve a single byte from a word.
-  | 0x1b => some .shl -- 0x1b / 2 / 1 / logical shift right operation.
-  | 0x1c => some .shr -- 0x1c / 2 / 1 / logical shift left operation.
-  | 0x1d => some .sar -- 0x1d / 2 / 1 / arithmetic (signed) shift right operation.
-  | 0x20 => some .kec -- 0x20 / 2 / 1 / compute Keccak-256 hash.
-  | 0x30 => some .address -- 0x30 / 0 / 1 / Get the address of the currently executing account.
-  | 0x31 => some .balance -- 0x31 / 1 / 1 / Get the balance of the specified account.
-  | 0x32 => some .origin -- 0x32 / 0 / 1 / Get the address that initiated the current transaction.
-  | 0x33 => some .caller -- 0x33 / 0 / 1 / Get the address that directly called the currently executing contract.
-  | 0x34 => some .callvalue -- 0x34 / 0 / 1 / Get the value (in wei) sent with the current transaction.
-  | 0x35 => some .calldataload -- 0x35 / 1 / 1 / Load input data from the current transaction.
-  | 0x36 => some .calldatasize -- 0x36 / 0 / 1 / Get the size of the input data from the current transaction.
-  | 0x37 => some .calldatacopy -- 0x37 / 3 / 0 / Copy input data from the current transaction to memory.
-  | 0x38 => some .codesize -- 0x38 / 0 / 1 / Get the size of the code of the currently executing contract.
-  | 0x39 => some .codecopy -- 0x39 / 3 / 0 / Copy the code of the currently executing contract to memory.
-  | 0x3a => some .gasprice -- 0x3a / 0 / 1 / Get the gas price of the current transaction.
-  | 0x3b => some .extcodesize -- 0x3b / 1 / 1 / Get the size of the code of an external account.
-  | 0x3c => some .extcodecopy -- 0x3c / 4 / 0 / Copy the code of an external account to memory.
-  | 0x3d => some .retdatasize -- 0x3d / 0 / 1 / Get the size of the output data from the previous call.
-  | 0x3e => some .retdatacopy -- 0x3e / 3 / 0 / Copy output data from the previous call to memory.
-  | 0x3f => some .extcodehash -- 0x3f / 1 / 1 / Get the code hash of an external account.
-  | 0x40 => some .blockhash -- 0x40 / 1 / 1 / get the hash of the specified block.
-  | 0x41 => some .coinbase -- 0x41 / 0 / 1 / get the address of the current block's miner.
-  | 0x42 => some .timestamp -- 0x42 / 0 / 1 / get the timestamp of the current block.
-  | 0x43 => some .number -- 0x43 / 0 / 1 / get the current block number.
-  | 0x44 => some .prevrandao -- 0x44 / 0 / 1 / get the difficulty of the current block.
-  | 0x45 => some .gaslimit -- 0x45 / 0 / 1 / get the gas limit of the current block.
-  | 0x46 => some .chainid -- 0x46 / 0 / 1 / get the chain id of the current blockchain.
-  | 0x47 => some .selfbalance -- 0x46 / 0 / 1 / get the chain id of the current blockchain.
-  | 0x48 => some .basefee -- 0x46 / 0 / 1 / get the chain id of the current blockchain.
-  | 0x50 => some .pop -- 0x50 / 1 / 0 / Remove an item from the stack.
-  | 0x51 => some .mload -- 0x51 / 1 / 1 / Load a word from memory.
-  | 0x52 => some .mstore -- 0x52 / 2 / 0 / Store a word in memory.
-  | 0x53 => some .mstore8 -- 0x53 / 2 / 0 / Store a byte in memory.
-  | 0x54 => some .sload -- 0x54 / 1 / 1 / Load a word from storage.
-  | 0x55 => some .sstore -- 0x55 / 2 / 0 / Store a word in storage.
-  | 0x58 => some .pc -- 0x58 / 0 / 1 / Get the current program counter value.
-  | 0x59 => some .msize -- 0x59 / 0 / 1 / Get the size of the memory.
-  | 0x5a => some .gas -- 0x5a / 0 / 1 / Get the amount of remaining gas.
-  | 0x80 => some (.dup 0)
-  | 0x81 => some (.dup 1)
-  | 0x82 => some (.dup 2)
-  | 0x83 => some (.dup 3)
-  | 0x84 => some (.dup 4)
-  | 0x85 => some (.dup 5)
-  | 0x86 => some (.dup 6)
-  | 0x87 => some (.dup 7)
-  | 0x88 => some (.dup 8)
-  | 0x89 => some (.dup 9)
-  | 0x8A => some (.dup 10)
-  | 0x8B => some (.dup 11)
-  | 0x8C => some (.dup 12)
-  | 0x8D => some (.dup 13)
-  | 0x8E => some (.dup 14)
-  | 0x8F => some (.dup 15)
-  | 0x90 => some (.swap 0)
-  | 0x91 => some (.swap 1)
-  | 0x92 => some (.swap 2)
-  | 0x93 => some (.swap 3)
-  | 0x94 => some (.swap 4)
-  | 0x95 => some (.swap 5)
-  | 0x96 => some (.swap 6)
-  | 0x97 => some (.swap 7)
-  | 0x98 => some (.swap 8)
-  | 0x99 => some (.swap 9)
-  | 0x9A => some (.swap 10)
-  | 0x9B => some (.swap 11)
-  | 0x9C => some (.swap 12)
-  | 0x9D => some (.swap 13)
-  | 0x9E => some (.swap 14)
-  | 0x9F => some (.swap 15)
-  | 0xA0 => some (.log 0)
-  | 0xA1 => some (.log 1)
-  | 0xA2 => some (.log 2)
-  | 0xA3 => some (.log 3)
-  | 0xA4 => some (.log 4)
-  | _ => none
-
-def B8.toXinst : B8 → Option Xinst
-  | 0xF0 => some .create
-  | 0xF1 => some .call
-  | 0xF2 => some .callcode
-  | 0xF4 => some .delcall
-  | 0xF5 => some .create2
-  | 0xFA => some .statcall
-  | _    => none
-
-def B8.toJinst : B8 → Option Jinst
-  | 0x56 => some .jump
-  | 0x57 => some .jumpi
-  | 0x5B => some .jumpdest
-  | _    => none
-
-def B8.toLinst : B8 → Option Linst
-  | 0x00 => some .stop
-  | 0xF3 => some .ret
-  | 0xFD => some .rev
-  | 0xFF => some .dest
-  | 0xFE => some .invalid
-  | _ => none
 
 inductive Ninst' : Type
   | reg : Rinst → Ninst'
@@ -1210,28 +426,6 @@ def getInst (υ : Var) (κ : Con)  : Option Inst' :=
     )
   else some (.last .stop)
 
--- def getInst (υ : Var) (κ : Con)  : Option Inst' :=
---   match κ.code.get? υ.pc with
---   | none => some (.last .stop)
---   | some b =>
---     (b.toRinst <&> (.next ∘ .reg)) <|>
---     (b.toXinst <&> (.next ∘ .exec)) <|>
---     (b.toJinst <&> .jump) <|>
---     (b.toLinst <&> .last) <|>
---     ( if h : 95 ≤ b.toNat ∧ b.toNat ≤ 127
---       then let len := b.toNat - 95
---            let slc := κ.code.sliceD (υ.pc + 1) len 0
---            let h_slc : slc.length ≤ 32 := by
---              simp [len, slc, Array.length_sliceD, h.right]
---            some (.next <| .push slc h_slc)
---       else none )
---
-def g_zero : Nat := 0
-def gVerylow : Nat := 3
-def gLow : Nat := 5
-def g_mid : Nat := 8
-def g_exp : Nat := 10
-def g_expbyte : Nat := 50
 
 def safeSub {ξ} [Sub ξ] [LE ξ] [@DecidableRel ξ (· ≤ ·)] (x y : ξ) : Option ξ :=
   if y ≤ x then some (x - y) else none
@@ -1318,6 +512,7 @@ def Sta.init : Sta := ⟨Array.mkArray 1024 (0 : B256), 0⟩
 
 -- need further update for precompiled contracts
 def θ.prep
+  (ω₀ : Wor)
   (H : Block)
   (ω : Wor)
   (A : Acs)
@@ -1349,6 +544,7 @@ def θ.prep
     | some aₛ => ω'₁.insert s {aₛ with bal := aₛ.bal - v}
   let cd : ByteArray := ω.code c
   let κ : Con := {
+    wor0 := ω₀
     cta := r, oga := o, gpr := p.toB256, cld := d
     cla := s, clv := v_app, code := cd, blk := H, exd := e, wup := w
   }
@@ -1377,27 +573,18 @@ def θ.wrap (wor : Wor) (acs : Acs) (Ξr : Ξ.Result) : theta.Result :=
   let o' : B8L := o.getD []
   ⟨ω', g', A', z, o'⟩
 
-def gColdSLoad : Nat := 2100
-def gSSet : Nat := 20000
-def gSReset : Nat := 2900
-def rSClear : Nat := 4800
 
-
-def B256.min : B256 → B256 → B256
-  | xs, ys => if xs ≤ ys then xs else ys
-instance : Min B256 := ⟨.min⟩
 
 def dataGas (cd : B8L) : Nat :=
   let aux : B8 → Nat := fun b => if b = 0 then 4 else 16
   (cd.map aux).sum
 
-def gTransaction : Nat := 21000
 
 def intrinsicGas (Rcv : Option Adr) (cd : B8L) (Ta : List (Adr × List B256)) : Nat :=
   let aux : (Adr × List B256) → Nat :=
-    fun | ⟨_, l⟩ => G_accesslistaddress + (G_accessliststorage * l.length)
+    fun | ⟨_, l⟩ => gAccesslistaddress + (gAccessliststorage * l.length)
   dataGas cd +
-  Rcv.rec (G_txcreate + initCodeCost cd) (fun _ => 0) +
+  Rcv.rec (gTxcreate + initCodeCost cd) (fun _ => 0) +
   gTransaction +
   (Ta.map aux).sum
 
@@ -1557,10 +744,10 @@ def Sta.popN (s : Sta ) : Nat → Option (List B256 × Sta)
     let (xs, s'') ← s'.popN n
     some ⟨x :: xs, s''⟩
 
-def sstoreStep (w₀ : Wor) (ω : Wor) (σ : Sta) (υ : Var) (κ : Con) :
+def sstoreStep (ω : Wor) (σ : Sta) (υ : Var) (κ : Con) :
     Option (Wor × Sta ×  Var) := do
   let (x, v', σ') ← σ.pop2
-  let (a₀ : Acct) ← w₀.find? κ.cta
+  let (a₀ : Acct) ← κ.wor0.find? κ.cta
   let (v₀ : B256) := ((a₀.stor.find? x).getD 0)
   let (a : Acct) ← ω.find? κ.cta
   let (v : B256) := ((a.stor.find? x).getD 0)
@@ -1609,66 +796,13 @@ def sstoreStep (w₀ : Wor) (ω : Wor) (σ : Sta) (υ : Var) (κ : Con) :
       }
     ⟩
 
-def List.swapCore {ξ} (x : ξ) : Nat → List ξ → Option (ξ × List ξ)
-  | 0, [] => none
-  | 0, y :: ys => some ⟨y, x :: ys⟩
-  | _ + 1, [] => none
-  | n + 1, y :: ys =>
-    match swapCore x n ys with
-    | some ⟨z, zs⟩ => some ⟨z, y :: zs⟩
-    | none => none
-
-def List.swap {ξ} (n : Nat) : List ξ → Option (List ξ)
-  | [] => none
-  | x :: xs =>
-    match swapCore x n xs with
-    | some ⟨y, ys⟩ => some (y :: ys)
-    | none => none
-
-def gBase : Nat := 2
 
 def memExp (s : Nat) (f l : B256) : Nat :=
   if l = 0
   then s
   else max s (ceilDiv (f.toNat + l.toNat) 32)
 
--- 'List.put xs n y z' is similar to 'List.set xs n y', except that
--- the former extends the input list (using the default filler 'z')
--- to ensure that 'y' is the 'n'th element of the resultant list.
-def List.put {ξ : Type u} : List ξ → Nat → ξ → ξ → List ξ
-  | _ :: xs, 0, y, _ => y :: xs
-  | [], 0, y, _ => [y]
-  | x :: xs, n + 1, y, z => x :: (List.put xs n y z)
-  | [], n + 1, y, z => z :: (List.put [] n y z)
 
-def List.puts {ξ : Type u} (xs : List ξ) (n : Nat) (ys : List ξ) (z : ξ) : List ξ :=
-  xs.takeD n z ++ ys ++ xs.drop (n + ys.length)
-
-def Array.writeD {ξ : Type u} (xs : Array ξ) (n : ℕ) : List ξ → Array ξ
-  | [] => xs
-  | y :: ys =>
-    if h : n < xs.size
-    then let xs' := xs.setN n y
-         writeD xs' (n + 1) ys
-    else xs
-
-def Array.copyD {ξ : Type u} (xs ys : Array ξ) : Array ξ :=
-  let f : (Array ξ × Nat) → ξ → (Array ξ × Nat) :=
-    λ ysn x => ⟨Array.setD ysn.fst ysn.snd x, ysn.snd + 1⟩
-  (Array.foldl f ⟨ys, 0⟩ xs).fst
-
-def Array.writeX {ξ : Type u} (xs : Array ξ) (n : ℕ) (ys : List ξ) (d : ξ) : Array ξ :=
-  if n + ys.length ≤ xs.size
-  then Array.writeD xs n ys
-  else let zs : Array ξ := Array.mkArray (n + ys.length) d
-       let zs' : Array ξ := Array.copyD xs zs
-       Array.writeD zs' n ys
-
-def gCopy : Nat := 3
-def gMemory : Nat := 3
-def gKeccak256 : Nat := 30
-def gKeccak256Word : Nat := 6
-def cMem (a : Nat) := gMemory * a + ((a ^ 2) / 512)
 
 def nextState (υ : Var) (cost : Nat)
   (act' : Option Nat := none)
@@ -1703,7 +837,7 @@ def Sta.toStringsCore (xs : Array B256) : Nat → List String
 def Sta.toStrings : Sta → List String
   | ⟨xs, n⟩ => Sta.toStringsCore xs n
 
-def Sta.toString (s : Sta) : String := Strings.join s.toStrings
+def Sta.toString (s : Sta) : String := String.joinln s.toStrings
 
 def Sta.swap : Sta → Nat → Option Sta
   | ⟨xs, n + 2⟩, k =>
@@ -1719,12 +853,6 @@ def Sta.dup : Sta → Nat → Option Sta
     else do let x ← xs.get? (n - (k + 1))
             Sta.push1 ⟨xs, n⟩ x
 
-def Linst.toB8 : Linst → B8
-  | .stop => 0x00
-  | .ret => 0xF3
-  | .rev => 0xFD
-  | .dest => 0xFF
-  | .invalid => 0xFE
 
 def pushItem (σ : Sta) (μ : Mem) (υ : Var) (x : B256) (c : Nat) :
     Option (Sta × Mem × Var) := do
@@ -1780,6 +908,7 @@ def Rinst.run (ω : Wor) (σ : Sta) (μ : Mem) (υ : Var) (κ : Con) :
   | .calldataload => do
     let (x, σ') ← σ.pop1
     let cd  ← B8L.toB256? (κ.cld.sliceD x.toNat 32 0)
+    -- dbg_trace s!"CALLDATA LOADED : {cd.toHex}"
     let σ'' ← σ'.push1 cd
     let υ' ← nextState υ gVerylow
     some ⟨σ'', μ, υ'⟩
@@ -1809,29 +938,33 @@ def Rinst.run (ω : Wor) (σ : Sta) (μ : Mem) (υ : Var) (κ : Con) :
     some ⟨σ'', μ, υ'⟩
   | .extcodecopy => do
     let (x, y, z, w, σ') ← σ.pop4
-    let cost := cAAccess x.toAdr υ.adrs + (gCopy * ceilDiv z.toNat 32)
-    let υ' ← nextState υ cost (act' := memExp υ.act y w)
-    let bs := κ.code.sliceD z.toNat w.toNat (Linst.toB8 .stop)
+    let a := x.toAdr
+    let cost := cAAccess x.toAdr υ.adrs + (gCopy * ceilDiv w.toNat 32)
+    let adrs' : AdrSet := υ.adrs.insert a
+    let υ' ← nextState υ cost (act' := memExp υ.act y w) (adrs' := adrs')
+    let cd : ByteArray := (ω.get a).code
+    let bs := cd.sliceD z.toNat w.toNat (Linst.toB8 .stop)
+    -- dbg_trace s!"EXTCODECOPY SOURCE ADDRESS : {a.toHex}"
+    -- dbg_trace s!"EXTCODECOPY VAL : {bs.toHex}"
     some ⟨σ', Array.writeX μ y.toNat bs 0, υ'⟩
   | .retdatasize => pushItem σ μ υ υ.ret.length.toB256 gBase
   | .retdatacopy => do
     let (x, y, z, σ') ← σ.pop3
-    let bs ← υ.ret.slice? y.toNat z.toNat
     let act' := memExp υ.act x z
-    checkRemGas υ (gVerylow + (gCopy * (ceilDiv z.toNat 32))) act'
     let υ' ← nextState υ (gVerylow + (gCopy * (ceilDiv z.toNat 32))) (act' := act')
+    let bs ← υ.ret.slice? y.toNat z.toNat
     some ⟨σ', Array.writeX μ x.toNat bs 0, υ'⟩
   | .extcodehash => do
     let (x, σ') ← σ.pop1
     let a := x.toAdr
     let adrs' := υ.adrs.insert a
+    let υ' ← nextState υ (cAAccess a υ.adrs) (adrs' := adrs')
     let hash : B256 :=
       if (Dead ω a)
       then 0
       else let cd := (ω.get a).code
            ByteArray.keccak 0 cd.size cd
     let σ'' ← σ'.push1 hash
-    let υ' ← nextState υ (cAAccess a υ.adrs) (adrs' := adrs')
     some ⟨σ'', μ, υ'⟩
   | .selfbalance => pushItem σ μ υ (ω.get κ.cta).bal gLow
   | .chainid => pushItem σ μ υ κ.blk.chainId gBase
@@ -1843,23 +976,22 @@ def Rinst.run (ω : Wor) (σ : Sta) (μ : Mem) (υ : Var) (κ : Con) :
   | .msize => pushItem σ μ υ (υ.act * 32).toB256 gBase
   | .mload => do
     let (x, σ') ← σ.pop1
+    let act' := memExp υ.act x (32 : Nat).toB256
+    let υ' ← nextState υ gVerylow (act' := act')
     let bs : B8L := μ.sliceD x.toNat 32 0
     let y : B256 ← B8L.toB256? bs
-    let act' := memExp υ.act x (32 : Nat).toB256
-    checkRemGas υ gVerylow act'
     let σ'' ← σ'.push1 y
-    let υ' ← nextState υ gVerylow (act' := act')
     some ⟨σ'', μ, υ'⟩
   | .mstore => do
     let (x, y, σ') ← σ.pop2
     let act' := memExp υ.act x (32 : Nat).toB256
-    checkRemGas υ gVerylow act'
     let υ' ← nextState υ gVerylow (act' := act')
+    -- dbg_trace s!"MSTORE LOC : {x.toHex}"
+    -- dbg_trace s!"MSTORE VAL : {y.toHex}"
     some ⟨σ', Array.writeX μ x.toNat y.toB8L 0, υ'⟩
   | .mstore8 => do
     let (x, y, σ') ← σ.pop2
     let act' := memExp υ.act x 1
-    checkRemGas υ gVerylow act'
     let υ' ← nextState υ gVerylow (act' := act')
     some ⟨σ', Array.writeX μ x.toNat [y.2.2.toUInt8] 0, υ'⟩
   | .gas => pushItem σ μ υ (υ.gas - gBase).toB256 gBase
@@ -1874,21 +1006,10 @@ def Rinst.run (ω : Wor) (σ : Sta) (μ : Mem) (υ : Var) (κ : Con) :
   | .or => applyBinary σ μ υ B256.or gVerylow
   | .xor => applyBinary σ μ υ B256.xor gVerylow
   | .signextend => applyBinary σ μ υ B256.signext gLow
-
-
-  -- | .pop => do
-  --   let (_, σ') ← σ.pop1
-  --   nextState μ σ' α (cost := gBase)
   | .pop => do
     let (_, σ') ← σ.pop1
     let υ' ← nextState υ gBase
     some ⟨σ', μ, υ'⟩
-
-  -- | .byte => do
-  --   let (x, y, σ') ← σ.pop2
-  --   let b : B8 := (List.getD y.toB8L x.toNat 0)
-  --   let σ'' ← σ'.push1 (b.toB256)
-  --   nextState μ σ'' α (cost := gVerylow)
   | .byte =>
     applyBinary σ μ υ (λ x y => (List.getD y.toB8L x.toNat 0).toB256) gVerylow
   | .shl => applyBinary σ μ υ (fun x y => y <<< x.toNat) gVerylow
@@ -1898,15 +1019,14 @@ def Rinst.run (ω : Wor) (σ : Sta) (μ : Mem) (υ : Var) (κ : Con) :
     let (x, y, σ') ← σ.pop2
     let act' := memExp υ.act x y
     let cost := gKeccak256 + (gKeccak256Word * (ceilDiv y.toNat 32))
-    checkRemGas υ cost act'
-    let σ'' ← σ'.push1 <| B8a.keccak x.toNat y.toNat μ
     let υ' ← nextState υ cost (act' := act')
+    let σ'' ← σ'.push1 <| B8a.keccak x.toNat y.toNat μ
     some ⟨σ'', μ, υ'⟩
   | .sub => applyBinary σ μ υ (· - ·) gVerylow
   | .mul => applyBinary σ μ υ (· * ·) gLow
   | .exp => do
     let (x, y, σ') ← σ.pop2
-    let cost := g_exp + (g_expbyte * y.bytecount)
+    let cost := gExp + (gExpbyte * y.bytecount)
     let σ'' ← σ'.push1 (B256.bexp x y)
     let υ' ← nextState υ cost
     some ⟨σ'', μ, υ'⟩
@@ -1915,8 +1035,8 @@ def Rinst.run (ω : Wor) (σ : Sta) (μ : Mem) (υ : Var) (κ : Con) :
   | .mod => applyBinary σ μ υ (· % ·) gLow
   | .smod => applyBinary σ μ υ B256.smod gLow
   | .add => applyBinary σ μ υ (· + ·) gVerylow
-  | .addmod => applyTernary σ μ υ B256.addmod g_mid
-  | .mulmod => applyTernary σ μ υ B256.mulmod g_mid
+  | .addmod => applyTernary σ μ υ B256.addmod gMid
+  | .mulmod => applyTernary σ μ υ B256.mulmod gMid
   | .swap n => do
     let σ' ← σ.swap n
     let υ' ← nextState υ gVerylow
@@ -1935,11 +1055,11 @@ def Rinst.run (ω : Wor) (σ : Sta) (μ : Mem) (υ : Var) (κ : Con) :
     some ⟨σ'', μ, υ'⟩
   | .pc => pushItem σ μ υ υ.pc.toB256 gBase
   | .log n => do
-    let (x, y, σ') ← σ.pop2
+    --let (x, y, σ') ← σ.pop2
+    let ⟨x :: y :: xs, σ'⟩ ← σ.popN (n + 2) | none
     let act' := memExp υ.act x y
     let cost := gLog + (gLogdata * y.toNat) + (n * gLogtopic)
     checkRemGas υ cost act'
-    let ⟨xs, σ''⟩ ← σ'.popN n
     let bs : B8L := μ.sliceD x.toNat y.toNat 0
     let log : RLP' :=
       .list [
@@ -1948,7 +1068,7 @@ def Rinst.run (ω : Wor) (σ : Sta) (μ : Mem) (υ : Var) (κ : Con) :
         .b8s bs
       ]
     let υ' ← nextState υ cost (act' := act') (logs' := log :: υ.logs)
-    some ⟨σ'', μ, υ'⟩
+    some ⟨σ', μ, υ'⟩
   | i => dbg_trace s!"UNIMPLEMENTED REGULAR INSTRUCTION EXECUTION : {i.toString}"; none
 
 
@@ -1960,9 +1080,6 @@ def Rinst.run (ω : Wor) (σ : Sta) (μ : Mem) (υ : Var) (κ : Con) :
 --       exceptional halting state due to the code byte that the program counter
 --       points to, or
 --   (2) recursion limit is reached (which should never happen with correct usage)
-
-def gHigh : Nat := 10
-def gJumpdest : Nat := 1
 
 def Acct.isEmpty (ac : Acct) : Prop :=
   ac.nonce = 0 ∧
@@ -1992,7 +1109,7 @@ def Jinst.run (σ : Sta) (υ : Var) (κ : Con) :
     some ⟨σ, {υ with gas := g', pc := υ.pc + 1}⟩
   | .jump => do
     let (loc, σ') ← σ.pop1
-    let g' ← safeSub υ.gas g_mid
+    let g' ← safeSub υ.gas gMid
     if jumpable' κ.code loc.toNat
     then some ⟨σ', {υ with gas := g', pc := loc.toNat}⟩
     else none
@@ -2005,8 +1122,7 @@ def Jinst.run (σ : Sta) (υ : Var) (κ : Con) :
          then some ⟨σ', {υ with gas := g', pc := loc.toNat}⟩
          else none
 
-def Ninst'.run (w₀ : Wor) (ω : Wor)
-    (σ : Sta) (μ : Mem) (υ : Var) (κ : Con) :
+def Ninst'.run (ω : Wor) (σ : Sta) (μ : Mem) (υ : Var) (κ : Con) :
     Ninst' → Option (Wor × Sta × Mem × Var)
   | .push x len => do
     let g' ← safeSub υ.gas (if len = 0 then gBase else gVerylow)
@@ -2015,7 +1131,7 @@ def Ninst'.run (w₀ : Wor) (ω : Wor)
     let υ' := {υ with gas := g', pc := υ.pc + len + 1}
     some ⟨ω, σ', μ, υ'⟩
   | .reg (.sstore) => do
-    let ⟨ω', σ', υ'⟩ ← sstoreStep w₀ ω σ υ κ --α ε
+    let ⟨ω', σ', υ'⟩ ← sstoreStep ω σ υ κ --α ε
     some ⟨ω', σ', μ, υ'⟩
   | .reg r => do
     let ⟨μ', σ', α'⟩ ← Rinst.run ω σ μ υ κ r --α ε r
@@ -2061,19 +1177,20 @@ def theta.Result.toState (ct : theta.Cont) (tr : theta.Result) :
   }
   some ⟨tr.wor, xs, Array.writeX ct.mem ct.olc.toNat cpy 0, υ'⟩
 
--- the X function of YP, except that the return type is modified to match
--- that of the Ξ function: the machine state (μ) returned by 'X' is never
--- used for anything except for remaining gas, so it is safe to discard the
--- unused information by the time X is returning.
--- This function returns 'none' only when either the recursion limit or an
--- unimplemented opcode is reached. returns 'some _' for all other cases.
--- return values :
+
+@[inline] def Char.isEq (c c' : Char) : Bool := c == c'
+
+@[inline] def Substring.trimLeftChar (s : Substring) (c : Char) : Substring :=
+  s.dropWhile (Char.isEq c)
+
+@[inline] def String.trimLeftChar (s : String) (c : Char) : String :=
+  (s.toSubstring.trimLeftChar c).toString
 
 def Ninst'.toString : Ninst' → String
   | reg o => Rinst.toString o
   | exec o => Xinst.toString o
   | push _ 0 => "PUSH0"
-  | push x len => "PUSH" ++ len.repr ++ " " ++ x.toHex
+  | push x len => "PUSH" ++ len.repr ++ " 0x" ++ (x.toHex.trimLeftChar '0')
 
 def Inst'.toString : Inst' → String
   | .next n => n.toString
@@ -2087,12 +1204,59 @@ def showLim (lim : Nat) (m : Var) : Option Unit :=
     return ()
   | _ => return ()
 
-def showExec (i : Inst') : Option Unit := do
-  dbg_trace s!"executing inst : {i.toString}"
+
+
+def showStep (υ : Var) (i : Inst') : Option Unit := do
+  -- let b : B8 := κ.code.get! υ.pc
+  dbg_trace (
+    "{" ++
+    s!"\"pc\": {υ.pc}, \"gas\": {υ.gas}, \"inst\": \"{i.toString}\"" ++
+    "}"
+  )
   return ()
 
-def exec (w₀ : Wor) :
-    Nat → Wor → Sta → Mem → Var → Con → Option Ξ.Result
+--structure Ξ.Result where
+--  (wor : Option Wor)
+--  (gas : Nat)
+--  (acs : Acs)
+--  (ret : Option B8L)
+
+
+def execSha (ω : Wor) (υ : Var) (κ : Con) : Ξ.Result :=
+  let g_r : Nat := 60 + (12 * (ceilDiv κ.cld.length 32))
+  match deductGas υ g_r with
+  | none => {wor := none, gas := 0, acs := υ.toAcs, ret := some []}
+  | some g' =>
+    let hash : B256 := B8L.sha256 κ.cld
+    {wor := some ω, gas := g', acs := υ.toAcs, ret := some hash.toB8L}
+
+-- the X function of YP, except that the return type is modified to match
+-- that of the Ξ function: the machine state (μ) returned by 'X' is never
+-- used for anything except for remaining gas, so it is safe to discard the
+-- unused information by the time X is returning.
+-- This function returns `none` only when either the recursion limit or an
+-- unimplemented opcode is reached. returns 'some _' for all other cases.
+-- in particular, exceptional halting state should not cause it to return
+-- a `none`.
+def mkThetaCont (ω : Wor) (σ' : Sta) (μ : Mem) (υ : Var)
+    (gas adr ilc isz olc osz : B256) : Option theta.Cont :=  do
+
+  let t : Adr := adr.toAdr
+  let act' : Nat := memExp (memExp υ.act ilc isz) olc osz
+  let memCost : Nat := cMem act' - cMem υ.act
+  let totalCost := (cCall ω υ gas.toNat memCost t 0) + memCost
+  let gas' ← safeSub υ.gas totalCost
+  some {
+    olc := olc
+    osz := osz
+    gas := gas'
+    mem := μ
+    pc := υ.pc
+    sta := σ'
+    act := act'
+  }
+
+def exec : Nat → Wor → Sta → Mem → Var → Con → Option Ξ.Result
   | 0, _, _, _, _, _ => none
   | lim + 1, ω, σ, μ, υ, κ  => do
     showLim lim υ
@@ -2100,7 +1264,7 @@ def exec (w₀ : Wor) :
     | none => some <| xhs υ
     | some i => do
       -- dbg_trace s!"remaining gas : {υ.gas}"
-      -- showExec i
+      -- showStep υ i
       -- dbg_trace s!"current stack :\n{Sta.toString σ}"
       match i with
       | .next (.exec .delcall) => do
@@ -2130,6 +1294,7 @@ def exec (w₀ : Wor) :
           then (theta.Result.toState bd ⟨ω, cg, A', 0, []⟩)
           else do let ⟨ω!, σ!, μ!, υ!, κ!⟩ :=
                         θ.prep
+                          κ.wor0
                           κ.blk
                           ω
                           A'
@@ -2144,15 +1309,26 @@ def exec (w₀ : Wor) :
                           i
                           (κ.exd - 1)
                           κ.wup
-                  let xr ← exec w₀ lim ω! σ! μ! υ! κ!
+                  let xr ←
+                    match κ!.cta.toNat with
+                    | 1 => dbg_trace "unimplemented : precompiled contract 1"; sorry
+                    | 2 => execSha ω! υ! κ!
+                    | 3 => dbg_trace "unimplemented : precompiled contract 3"; sorry
+                    | 4 => dbg_trace "unimplemented : precompiled contract 4"; sorry
+                    | 5 => dbg_trace "unimplemented : precompiled contract 5"; sorry
+                    | 6 => dbg_trace "unimplemented : precompiled contract 6"; sorry
+                    | 7 => dbg_trace "unimplemented : precompiled contract 7"; sorry
+                    | 8 => dbg_trace "unimplemented : precompiled contract 8"; sorry
+                    | 9 => dbg_trace "unimplemented : precompiled contract 9"; sorry
+                    | _ => exec lim ω! σ! μ! υ! κ!
                   let θr := θ.wrap ω! υ!.toAcs xr
                   (theta.Result.toState bd θr)
-        exec w₀ lim ω? σ? μ? υ? κ
+        exec lim ω? σ? μ? υ? κ
       | .next (.exec .call) => do
         let (gas, adr, clv, ilc, isz, olc, osz, σ') ← σ.pop7
-        let i : B8L := μ.sliceD ilc.toNat isz.toNat 0
         let t : Adr := adr.toAdr
         -- dbg_trace s!"nested call to address : {t.toHex}"
+        let i : B8L := μ.sliceD ilc.toNat isz.toNat 0
         let as' : AdrSet := υ.adrs.insert t
         let A' : Acs := {υ.toAcs with adrs := as'}
         let act' : Nat := memExp (memExp υ.act ilc isz) olc osz
@@ -2173,8 +1349,9 @@ def exec (w₀ : Wor) :
         let ⟨ω?, σ?, μ?, υ?⟩ ←
           if 0 = κ.exd ∨ (ω.get κ.cta).bal < clv
           then (theta.Result.toState bd ⟨ω, cg, A', 0, []⟩)
-          else do let ⟨ω!, σ!, μ!, υ!, κ!⟩  : (Wor × Sta × Mem × Var × Con) :=
+          else do let ⟨ω!, σ!, μ!, υ!, κ!⟩ : (Wor × Sta × Mem × Var × Con) :=
                         θ.prep
+                          κ.wor0
                           κ.blk
                           ω
                           A'
@@ -2189,19 +1366,29 @@ def exec (w₀ : Wor) :
                           i
                           (κ.exd - 1)
                           κ.wup
-                  -- dbg_trace s!"code of nested delcall : {B8L.toHex s'.env.code.toList}"
-                  let xr ← exec w₀ lim ω! σ! μ! υ! κ!
+                  let xr ←
+                    match κ!.cta.toNat with
+                    | 1 => dbg_trace "unimplemented : precompiled contract 1"; sorry
+                    | 2 => execSha ω! υ! κ!
+                    | 3 => dbg_trace "unimplemented : precompiled contract 3"; sorry
+                    | 4 => dbg_trace "unimplemented : precompiled contract 4"; sorry
+                    | 5 => dbg_trace "unimplemented : precompiled contract 5"; sorry
+                    | 6 => dbg_trace "unimplemented : precompiled contract 6"; sorry
+                    | 7 => dbg_trace "unimplemented : precompiled contract 7"; sorry
+                    | 8 => dbg_trace "unimplemented : precompiled contract 8"; sorry
+                    | 9 => dbg_trace "unimplemented : precompiled contract 9"; sorry
+                    | _ => exec lim ω! σ! μ! υ! κ!
                   let θr := θ.wrap ω! υ!.toAcs xr
                   (theta.Result.toState bd θr)
-        exec w₀ lim ω? σ? μ? υ? κ
+        exec lim ω? σ? μ? υ? κ
       | .next n =>
-        match n.run w₀ ω σ μ υ κ  with
+        match n.run ω σ μ υ κ  with
         | none => some (xhs υ)
-        | some ⟨ω', σ', μ', υ'⟩ => exec w₀ lim ω' σ' μ' υ' κ --s'.env s'.acr s'.wor s'.mcn
+        | some ⟨ω', σ', μ', υ'⟩ => exec lim ω' σ' μ' υ' κ --s'.env s'.acr s'.wor s'.mcn
       | .jump j =>
          match j.run σ υ κ with
          | none => some (xhs υ)
-         | some ⟨σ', υ'⟩ => exec w₀ lim ω σ' μ υ' κ
+         | some ⟨σ', υ'⟩ => exec lim ω σ' μ υ' κ
       | .last .stop => some {wor := ω, gas := υ.gas, acs := υ.toAcs, ret := some []}
       | .last .ret => some <| (retRun ω σ μ υ).getD (xhs υ)
       | .last .dest => do
@@ -2255,8 +1442,8 @@ def theta
   (e : Nat)
   (w : Bool) :
   Option theta.Result :=
-  let ⟨ω?, σ?, μ?, υ?, κ?⟩ := θ.prep H ω A s o r c g p v v_app d e w
-  match exec ω₀ g ω? σ? μ? υ? κ? with
+  let ⟨ω?, σ?, μ?, υ?, κ?⟩ := θ.prep ω₀ H ω A s o r c g p v v_app d e w
+  match exec g ω? σ? μ? υ? κ? with
   | none => none
   | some xr => some (θ.wrap ω? υ?.toAcs xr)
 
@@ -2268,82 +1455,11 @@ def publicAddress (hsa : ByteArray) (ri : UInt8) (rsa : ByteArray) : IO Adr :=
     then IO.throw "ecrecover failed"
     else (B8L.toAdr pa).toIO "bytearray to address conversion failed"
 
-def IO.guard (φ : Prop) [Decidable φ] (msg : String) : IO Unit :=
-  if φ then return () else IO.throw msg
-
-inductive TxType : Type
-  | zero : TxType
-  -- access list (T_A)
-  | one : AccessList → TxType
-  -- access list (T_A), max fee per gas (T_m), max priority fee per gas (T_f)
-  | two : AccessList → B256 → B256 → TxType
-
-structure TxBytesContent : Type where
-  (chainId : Option Nat)
-  (yParity : Bool)
-  (type : TxType)
-  (nonce : B256)
-  (gasPrice : B256)
-  (gasLimit : B256)
-  (receiver : Adr)
-  (val : B256)
-  (calldata : B8L)
-  (r : B8L)
-  (s : B8L)
-  (acc : AccessList)
-
 structure transact.Result : Type where
   (wor : Wor)
   (gas : Nat)
   (log : B256)
   (sta : Bool)
-
-def decodeTxBytes (tbs : B8L) : IO (TxBytesContent × B256) :=
-  match RLP'.decode tbs with
-  | RLP'.list [
-      .b8s nonce,
-      .b8s gasPrice,
-      .b8s gasLimit,
-      .b8s receiver,
-      .b8s val,
-      .b8s calldata,
-      .b8s [v],
-      .b8s r,
-      .b8s s
-    ] => do
-    let bs :=
-      RLP'.encode <|
-        .list [
-          .b8s nonce,
-          .b8s gasPrice,
-          .b8s gasLimit,
-          .b8s receiver,
-          .b8s val,
-          .b8s calldata
-        ]
-    let recAdr ← (B8L.toAdr receiver).toIO "cannot convert bytes to receiver address"
-    return ⟨
-      {
-        chainId := none
-        yParity := if (v - 0x1B) = 0 then 0 else 1
-        type := .zero
-        nonce    := nonce.toB256P
-        gasPrice := gasPrice.toB256P
-        gasLimit := gasLimit.toB256P
-        receiver := recAdr
-        val := val.toB256P
-        calldata := calldata
-        r := (r.reverse.takeD 32 0).reverse
-        s := (s.reverse.takeD 32 0).reverse
-        acc := []
-      },
-      bs.keccak
-    ⟩
-  | _ => IO.throw "Error : TX bytes decoding failed"
-
-def eqTest {ξ} [DecidableEq ξ] (x y : ξ) (testName : String) : IO Unit := do
-  .guard (x = y) (testName ++ " : fail")
-  .println (testName ++ " : pass")
 
 def eraseIfEmpty (w : Wor) (a : Adr) : Wor := w.set a <| w.get a
 
@@ -2402,8 +1518,6 @@ def Tx.run
     sta := tr.status
   }
 
-def String.joinnl (l : List String) : String :=
-  l.foldl (fun r s => r ++ "\n" ++ s) ""
 
 def Test.run (t : Test) : IO Unit := do
   let ⟨tx, hsh⟩ ← decodeTxBytes t.txdata
@@ -2413,7 +1527,7 @@ def Test.run (t : Test) : IO Unit := do
   let sender ← publicAddress hsa ri rsa
 
   .println "initial world : "
-  .println (Strings.join t.world.toStrings)
+  .println (String.joinln t.world.toStrings)
 
   let sa₀ ← (t.world.find? sender).toIO "no sender account"
 
@@ -2441,6 +1555,8 @@ def Test.run (t : Test) : IO Unit := do
   .guard (tx.calldata = t.calldata) "calldata check : fail"
   .println "calldata check : pass"
 
+  .println s!"CALLDATA : {tx.calldata.toHex}"
+
   let rst ←
     Tx.run
       {
@@ -2458,7 +1574,7 @@ def Test.run (t : Test) : IO Unit := do
 
   .println s!"tx status : {rst.sta}"
   .println "world state after tx :"
-  .println (Strings.join rst.wor.toStrings)
+  .println (String.joinln rst.wor.toStrings)
 
   let temp' := (List.map toKeyVal rst.wor.toList)
   let finalNTB : NTB := Lean.RBMap.fromList temp' _
@@ -2486,7 +1602,7 @@ def main : List String → IO Unit
     let j ← readJsonFile testPath
     let td ← Lean.Json.toTestData j
     let ts ← getTests td
-    Tests.run 1 ts
+    Tests.run 0 ts
   | [testPath, testNum] => do
     let n ← testNum.toNat?.toIO "error : second argument is not a number"
     let j ← readJsonFile testPath
@@ -2494,3 +1610,13 @@ def main : List String → IO Unit
     let ts ← getTests td
     ((ts.get? n).toIO s!"test #{n} does not exist") >>= Test.run
   | _ => IO.throw "error : invalid arguments"
+
+
+-- def Bytes.toHexLine (bs : Bytes) : String :=
+--   s!"hex\"{bs.toHex}\""
+--
+-- def WethByteCode : String :=
+--   List.foldr
+--      (λ s0 s1 => s0 ++ "\n" ++ s1)
+--      "" <| List.map Bytes.toHexLine
+--         <| List.chunks 31 <| Option.getD weth.compile []
