Blanc/Common.lean
@@ -3795,3 +3795,160 @@ lemma le_of_increase {m n : ℕ} {k : Bits m} {v : Bits n} {f g : Bits m → Bit
     have h_rw : f k + v = g k := (h k).left rfl
     rw [← h_rw]; apply Bits.le_add_right h'
   · rw [(h k').right h_eq]; apply Bits.le_refl
+
+def B8.toRinst : B8 → Option Rinst
+  | 0x01 => some .add -- 0x01 / 2 / 1 / addition operation.
+  | 0x02 => some .mul -- 0x02 / 2 / 1 / multiplication operation.
+  | 0x03 => some .sub -- 0x03 / 2 / 1 / subtraction operation.
+  | 0x04 => some .div -- 0x04 / 2 / 1 / integer division operation.
+  | 0x05 => some .sdiv -- 0x05 / 2 / 1 / signed integer division operation.
+  | 0x06 => some .mod -- 0x06 / 2 / 1 / modulo operation.
+  | 0x07 => some .smod -- 0x07 / 2 / 1 / signed modulo operation.
+  | 0x08 => some .addmod -- 0x08 / 3 / 1 / modulo addition operation.
+  | 0x09 => some .mulmod -- 0x09 / 3 / 1 / modulo multiplication operation.
+  | 0x0a => some .exp -- 0x0a / 2 / 1 / exponentiation operation.
+  | 0x0b => some .signextend -- 0x0b / 2 / 1 / sign extend operation.
+  | 0x10 => some .lt -- 0x10 / 2 / 1 / less-than comparison.
+  | 0x11 => some .gt -- 0x11 / 2 / 1 / greater-than comparison.
+  | 0x12 => some .slt -- 0x12 / 2 / 1 / signed less-than comparison.
+  | 0x13 => some .sgt -- 0x13 / 2 / 1 / signed greater-than comparison.
+  | 0x14 => some .eq -- 0x14 / 2 / 1 / equality comparison.
+  | 0x15 => some .iszero -- 0x15 / 1 / 1 / tests if the input is zero.
+  | 0x16 => some .and -- 0x16 / 2 / 1 / bitwise and operation.
+  | 0x17 => some .or -- 0x17 / 2 / 1 / bitwise or operation.
+  | 0x18 => some .xor -- 0x18 / 2 / 1 / bitwise xor operation.
+  | 0x19 => some .not -- 0x19 / 1 / 1 / bitwise not operation.
+  | 0x1a => some .byte -- 0x1a / 2 / 1 / retrieve a single byte from a word.
+  | 0x1b => some .shl -- 0x1b / 2 / 1 / logical shift right operation.
+  | 0x1c => some .shr -- 0x1c / 2 / 1 / logical shift left operation.
+  | 0x1d => some .sar -- 0x1d / 2 / 1 / arithmetic (signed) shift right operation.
+  | 0x20 => some .kec -- 0x20 / 2 / 1 / compute Keccak-256 hash.
+  | 0x30 => some .address -- 0x30 / 0 / 1 / Get the address of the currently executing account.
+  | 0x31 => some .balance -- 0x31 / 1 / 1 / Get the balance of the specified account.
+  | 0x32 => some .origin -- 0x32 / 0 / 1 / Get the address that initiated the current transaction.
+  | 0x33 => some .caller -- 0x33 / 0 / 1 / Get the address that directly called the currently executing contract.
+  | 0x34 => some .callvalue -- 0x34 / 0 / 1 / Get the value (in wei) sent with the current transaction.
+  | 0x35 => some .calldataload -- 0x35 / 1 / 1 / Load input data from the current transaction.
+  | 0x36 => some .calldatasize -- 0x36 / 0 / 1 / Get the size of the input data from the current transaction.
+  | 0x37 => some .calldatacopy -- 0x37 / 3 / 0 / Copy input data from the current transaction to memory.
+  | 0x38 => some .codesize -- 0x38 / 0 / 1 / Get the size of the code of the currently executing contract.
+  | 0x39 => some .codecopy -- 0x39 / 3 / 0 / Copy the code of the currently executing contract to memory.
+  | 0x3a => some .gasprice -- 0x3a / 0 / 1 / Get the gas price of the current transaction.
+  | 0x3b => some .extcodesize -- 0x3b / 1 / 1 / Get the size of the code of an external account.
+  | 0x3c => some .extcodecopy -- 0x3c / 4 / 0 / Copy the code of an external account to memory.
+  | 0x3d => some .retdatasize -- 0x3d / 0 / 1 / Get the size of the output data from the previous call.
+  | 0x3e => some .retdatacopy -- 0x3e / 3 / 0 / Copy output data from the previous call to memory.
+  | 0x3f => some .extcodehash -- 0x3f / 1 / 1 / Get the code hash of an external account.
+  | 0x40 => some .blockhash -- 0x40 / 1 / 1 / get the hash of the specified block.
+  | 0x41 => some .coinbase -- 0x41 / 0 / 1 / get the address of the current block's miner.
+  | 0x42 => some .timestamp -- 0x42 / 0 / 1 / get the timestamp of the current block.
+  | 0x43 => some .number -- 0x43 / 0 / 1 / get the current block number.
+  | 0x44 => some .prevrandao -- 0x44 / 0 / 1 / get the difficulty of the current block.
+  | 0x45 => some .gaslimit -- 0x45 / 0 / 1 / get the gas limit of the current block.
+  | 0x46 => some .chainid -- 0x46 / 0 / 1 / get the chain id of the current blockchain.
+  | 0x47 => some .selfbalance -- 0x46 / 0 / 1 / get the chain id of the current blockchain.
+  | 0x48 => some .basefee -- 0x46 / 0 / 1 / get the chain id of the current blockchain.
+  | 0x50 => some .pop -- 0x50 / 1 / 0 / Remove an item from the stack.
+  | 0x51 => some .mload -- 0x51 / 1 / 1 / Load a word from memory.
+  | 0x52 => some .mstore -- 0x52 / 2 / 0 / Store a word in memory.
+  | 0x53 => some .mstore8 -- 0x53 / 2 / 0 / Store a byte in memory.
+  | 0x54 => some .sload -- 0x54 / 1 / 1 / Load a word from storage.
+  | 0x55 => some .sstore -- 0x55 / 2 / 0 / Store a word in storage.
+  | 0x58 => some .pc -- 0x58 / 0 / 1 / Get the current program counter value.
+  | 0x59 => some .msize -- 0x59 / 0 / 1 / Get the size of the memory.
+  | 0x5a => some .gas -- 0x5a / 0 / 1 / Get the amount of remaining gas.
+  | 0x80 => some (.dup 0)
+  | 0x81 => some (.dup 1)
+  | 0x82 => some (.dup 2)
+  | 0x83 => some (.dup 3)
+  | 0x84 => some (.dup 4)
+  | 0x85 => some (.dup 5)
+  | 0x86 => some (.dup 6)
+  | 0x87 => some (.dup 7)
+  | 0x88 => some (.dup 8)
+  | 0x89 => some (.dup 9)
+  | 0x8A => some (.dup 10)
+  | 0x8B => some (.dup 11)
+  | 0x8C => some (.dup 12)
+  | 0x8D => some (.dup 13)
+  | 0x8E => some (.dup 14)
+  | 0x8F => some (.dup 15)
+  | 0x90 => some (.swap 0)
+  | 0x91 => some (.swap 1)
+  | 0x92 => some (.swap 2)
+  | 0x93 => some (.swap 3)
+  | 0x94 => some (.swap 4)
+  | 0x95 => some (.swap 5)
+  | 0x96 => some (.swap 6)
+  | 0x97 => some (.swap 7)
+  | 0x98 => some (.swap 8)
+  | 0x99 => some (.swap 9)
+  | 0x9A => some (.swap 10)
+  | 0x9B => some (.swap 11)
+  | 0x9C => some (.swap 12)
+  | 0x9D => some (.swap 13)
+  | 0x9E => some (.swap 14)
+  | 0x9F => some (.swap 15)
+  | 0xA0 => some (.log 0)
+  | 0xA1 => some (.log 1)
+  | 0xA2 => some (.log 2)
+  | 0xA3 => some (.log 3)
+  | 0xA4 => some (.log 4)
+  | _ => none
+
+def B8.toXinst : B8 → Option Xinst
+  | 0xF0 => some .create
+  | 0xF1 => some .call
+  | 0xF2 => some .callcode
+  | 0xF4 => some .delcall
+  | 0xF5 => some .create2
+  | 0xFA => some .statcall
+  | _    => none
+
+def B8.toJinst : B8 → Option Jinst
+  | 0x56 => some .jump
+  | 0x57 => some .jumpi
+  | 0x5B => some .jumpdest
+  | _    => none
+
+def B8.toLinst : B8 → Option Linst
+  | 0x00 => some .stop
+  | 0xF3 => some .ret
+  | 0xFD => some .rev
+  | 0xFF => some .dest
+  | 0xFE => some .invalid
+  | _ => none
+
+def Jinst.toB8 : Jinst → B8
+  | jump => 0x56     -- 0x56 / 1 / 0 / Unconditional jump.
+  | jumpi => 0x57    -- 0x57 / 2 / 0 / Conditional jump.
+  | jumpdest => 0x5B -- 0x5b / 0 / 0 / Mark a valid jump destination.
+
+def Linst.toB8 : Linst → B8
+  | .stop => 0x00
+  | .ret => 0xF3
+  | .rev => 0xFD
+  | .dest => 0xFF
+  | .invalid => 0xFE
+
+def Adr.toHex (a : Adr) : String :=
+  a.high.toHex ++ a.mid.toHex ++ a.low.toHex
+
+
+def B8L.toAdr : B8L → Option Adr
+  | x0 :: x1 :: x2 :: x3 ::
+    y0 :: y1 :: y2 :: y3 ::
+    y4 :: y5 :: y6 :: y7 ::
+    z0 :: z1 :: z2 :: z3 ::
+    z4 :: z5 :: z6 :: z7 :: _ =>
+    some ⟨
+      B8s.toB32 x0 x1 x2 x3,
+      B8s.toB64 y0 y1 y2 y3 y4 y5 y6 y7,
+      B8s.toB64 z0 z1 z2 z3 z4 z5 z6 z7,
+    ⟩
+  | _ => none
+
+def Hex.toAdr (hx : String) : Option Adr := Hex.toB8L hx >>= B8L.toAdr
+
+def Adr.toB8L (a : Adr) : B8L :=
+  a.high.toB8L ++ a.mid.toB8L ++ a.low.toB8L
