Blanc/TestParse.lean
@@ -1,0 +1,463 @@
+import Lean.Data.Json
+import Lean.Data.Json.Parser
+import Blanc.Common
+
+structure EnvData where
+  (baseFee : B256)
+  (coinbase : Adr)
+  (prevRandao : B256)
+  (blockGasLimit : B256)
+  (timestamp : B256)
+  (number : B256)
+
+structure PreData where
+  (addr : Adr)
+  (nonce : B8L)
+  (bal : B8L)
+  (stor : Stor)
+  (code : B8L)
+
+structure PostData where
+  (hash : B256)
+  (dataIdx : Nat)
+  (gasIdx : Nat)
+  (valueIdx : Nat)
+  (logs : B256)
+  (txdata : B8L)
+
+structure TransactionData : Type where
+  (data : List B8L)
+  (gasLimit : List B256)
+  (gasPrice : B256)
+  (nonce : B256)
+  (secretKey : B256)
+  (sender : Adr)
+  (receiver : Adr)
+  (value : List B256)
+
+structure TestData where
+  (info : Lean.Json)
+  (env  : EnvData)
+  (pre  : List PreData)
+  (post : String × List PostData)
+  (tx   : TransactionData)
+
+def readJsonFile (filename : System.FilePath) : IO Lean.Json := do
+  let contents ← IO.FS.readFile filename
+  match Lean.Json.parse contents with
+  | .ok json => pure json
+  | .error err => throw (IO.userError err)
+
+mutual
+  partial def StringJsons.toStrings : List ((_ : String) × Lean.Json) → List String
+    | [] => []
+    | sj :: sjs =>
+      (sj.fst :: Lean.Json.toStrings sj.snd) ++ StringJsons.toStrings sjs
+
+  partial def Lean.Jsons.toStrings : List Lean.Json → List String
+    | [] => []
+    | j :: js => Lean.Json.toStrings j ++ Lean.Jsons.toStrings js
+
+  partial def Lean.Json.toStrings : Lean.Json → List String
+    | .null => ["null"]
+    | .bool b => [s!"bool : {b}"]
+    | .num n => [s!"num : {n}"]
+    | .str s => [s!"str : {s}"]
+    | .arr js =>
+      "arr :" :: (Lean.Jsons.toStrings js.toList).map ("  " ++ ·)
+    | .obj m => do
+      let kvs := m.toArray.toList
+      "obj : " :: (StringJsons.toStrings kvs).map ("  " ++ ·)
+end
+
+def Lean.Json.toString (j : Lean.Json) : String := String.joinln j.toStrings
+
+
+def List.chunksCore {ξ} (m : Nat) : Nat → List ξ → List (List ξ)
+  | _, [] => [[]]
+  | 0, x :: xs =>
+    match chunksCore m m xs with
+    | [] => [[], [x]]
+    | ys :: yss => [] :: (x :: ys) :: yss
+  | n + 1, x :: xs =>
+    match chunksCore m n xs with
+    | [] => [[x]]
+    | ys :: yss => (x :: ys) :: yss
+
+def List.chunks {ξ} (m : Nat) : List ξ → List (List ξ) := List.chunksCore m (m + 1)
+
+def longB8LToStrings (hd : String) (bs : B8L) : List String :=
+  match List.chunks 31 bs with
+  | [] => [hd]
+  | [bs'] => [s!"{hd} : {B8L.toHex bs'}"]
+  | bss => s!"{hd} :" :: bss.map (λ bs' => pad (B8L.toHex bs'))
+
+def txdataToStrings (tx : B8L) : List String :=
+  match List.chunks 31 tx with
+  | [] => ["txdata :"]
+  | [bs] => [s!"txdata : {B8L.toHex bs}"]
+  | bss => "txdata :" :: bss.map (λ bs => pad (B8L.toHex bs))
+
+def postAcct.toStrings (p : PostData) : List String :=
+  fork "Post Acct" [
+    [s!"hash : {p.hash.toHex}"],
+    [s!"data index : {p.dataIdx}"],
+    [s!"gas index : {p.gasIdx}"],
+    [s!"value index : {p.valueIdx}"],
+    [s!"logs : {B256.toHex p.logs}"],
+    txdataToStrings p.txdata
+  ]
+
+def Lean.RBMap.toStrings {α β cmp} (m : Lean.RBMap α β cmp)
+  (fmt : α × β → List String): List String :=
+  let kvs := m.toArray.toList
+  fork "map" (kvs.map fmt)
+
+def Stor.toStrings (s : Stor) : List String :=
+  let kvs := s.toArray.toList
+  let kvToStrings : B256 × B256 → List String :=
+    λ nb => [s!"{B256.toHex nb.fst} : {B256.toHex nb.snd}"]
+  fork "stor" (kvs.map kvToStrings)
+
+def preAcct.toStrings (p : PreData) : List String :=
+  fork "Pre Acct" [
+    [s!"address : {p.addr.toHex}"],
+    [s!"nonce : {B8L.toHex p.nonce}"],
+    [s!"balance : {B8L.toHex p.bal}"],
+    p.stor.toStrings,
+    [s!"code : {B8L.toHex p.code}"]
+  ]
+
+def postToStrings : (String × List PostData) → List String
+  | ⟨s, ps⟩ => fork "Post" [[s], listToStrings postAcct.toStrings ps]
+
+def EnvData.toStrings (e : EnvData) : List String :=
+  fork "env" [
+    [s!"coinbase : {e.coinbase.toHex}"],
+  ]
+
+def preToStrings (l : List PreData) : List String :=
+  fork "pre" [listToStrings preAcct.toStrings l]
+
+def TransactionData.toStrings (tx : TransactionData) : List String :=
+  fork "transaction" [
+    fork "data" [listToStrings (λ x => [B8L.toHex x]) tx.data],
+    fork "gasLimit" [listToStrings (λ x => [x.toHex]) tx.gasLimit],
+    [s!"gasPrice : {tx.gasPrice.toHex}"],
+    [s!"nonce :     {tx.nonce.toHex}"],
+    [s!"secretKey : {tx.secretKey.toHex}"],
+    [s!"sender : {tx.sender.toHex}"],
+    [s!"to : {tx.receiver.toHex}"],
+    fork "value" [listToStrings (λ x => [x.toHex]) tx.value]
+  ]
+
+structure Test where
+  (baseFee : B256)
+  (coinbase : Adr)
+  (prevRandao : B256)
+  (blockGasLimit : B256)
+  (number : B256)
+  (timestamp : B256)
+  (world  : Wor)
+  (txdata : B8L)
+  (nonce : B256)
+  (gasPrice : B256)
+  (gasLimit : B256)
+  (sender : Adr)
+  (receiver : Adr)
+  (value : B256)
+  (calldata : B8L)
+  (hash : B256) -- ?
+  (logs : B256) -- keccak hash of (RLP-encoded) log items
+  (secret : B256)
+
+def Acct.toStrings (s : String) (a : Acct) : List String :=
+  fork s [
+    [s!"nonce : 0x{a.nonce.toHex}"],
+    [s!"bal : 0x{a.bal.toHex}"],
+    a.stor.toStrings,
+    longB8LToStrings "code" a.code.toList
+  ]
+
+
+def Wor.toStrings (w : Wor) : List String :=
+  let kvs := w.toArray.toList
+  let kvToStrings : Adr × Acct → List String :=
+    fun x => Acct.toStrings x.fst.toHex x.snd
+  fork "world" (kvs.map kvToStrings)
+
+def Test.toStrings (t : Test) : List String :=
+  fork "VM Test" [
+    [s!"coinbase : {t.coinbase.toHex}"],
+    t.world.toStrings,
+    txdataToStrings t.txdata,
+    [s!"nonce : 0x{t.nonce.toHex}"],
+    [s!"gas price : 0x{t.gasPrice.toHex}"],
+    [s!"gas limit : 0x{t.gasLimit.toHex}"],
+    [s!"sender : 0x{t.sender.toHex}"],
+    [s!"receiver : 0x{t.receiver.toHex}"],
+    [s!"value : 0x{t.value.toHex}"],
+    longB8LToStrings "calldata" t.calldata,
+    [s!"hash : 0x{t.hash.toHex}"],
+    [s!"logs : 0x{t.logs.toHex}"],
+    [s!"secret : 0x{t.secret.toHex}"]
+  ]
+
+def TestData.toStrings (t : TestData) : List String :=
+  fork "VM Test" [
+    ["info ..."],--t.info.toStrings,
+    EnvData.toStrings t.env,
+    preToStrings t.pre,
+    postToStrings t.post,
+    t.tx.toStrings
+  ]
+
+def TestData.toString (t : TestData) : String := String.joinln t.toStrings
+def Test.toString (t : Test) : String := String.joinln t.toStrings
+
+def Lean.Json.fromArr : Lean.Json → IO (List Json)
+  | .arr a => return a.toList
+  | _ => IO.throw "not an array"
+
+def Lean.Json.fromObj : Lean.Json → IO (RBNode String (λ _ => Json))
+  | .obj r => return r
+  | _ => IO.throw "not an object"
+
+def Lean.Json.fromStr : Lean.Json → IO String
+  | .str s => return s
+  | _ => IO.throw "not a string"
+
+def Lean.Json.fromNum : Lean.Json → IO JsonNumber
+  | .num n => return n
+  | _ => IO.throw "not a string"
+
+def Lean.JsonNumber.toNat : JsonNumber → IO Nat
+  | ⟨.ofNat x, 0⟩ => return x
+  | ⟨.negSucc _, _⟩ => IO.throw "negative mantissa"
+  | ⟨_, e + 1⟩ => IO.throw s!"nonzero exponent : {e + 1}"
+
+def Lean.Json.fromSingleton : Lean.Json → IO (String × Lean.Json)
+  | .obj (.node _ .leaf k v .leaf) => return ⟨k, v⟩
+  | _ => IO.throw "not a singleton"
+
+
+def Lean.Json.toPostData : Json → IO PostData
+  | .obj r => do
+    let hsx ← (r.find compare "hash").toIO "cannot retrieve hash bytes" >>= fromStr >>= Hex.from0x
+    let hs ← (Hex.toB256? hsx).toIO "cannot convert hash bytes to word"
+    let lgx ← (r.find compare "logs").toIO "cannot get logs bytes" >>= fromStr >>= Hex.from0x
+    let lg ← (Hex.toB256? lgx).toIO "cannot convert logs bytes to word"
+    let txx ← (r.find compare "txbytes").toIO "cannot get tx bytes" >>= fromStr >>= Hex.from0x
+    let tx ← (Hex.toB8L txx).toIO "cannot convert tx bytes to word"
+    let dgv ← (r.find compare "indexes").toIO "cannot get indexes" >>= Json.fromObj
+    let d ← (dgv.find compare "data").toIO "cannot get data" >>= Json.fromNum >>= JsonNumber.toNat
+    let g ← (dgv.find compare "gas").toIO "cannot get gas" >>= Json.fromNum >>= JsonNumber.toNat
+    let v ← (dgv.find compare "value").toIO "cannot get value" >>= Json.fromNum >>= JsonNumber.toNat
+    return ⟨hs, d, g, v, lg, tx⟩
+  | _ => IO.throw "Json-to-PostData failed"
+
+def Lean.Json.toB8L (j : Json) : IO B8L := do
+  let x ← fromStr j >>= Hex.from0x
+  (Hex.toB8L x).toIO ""
+
+def Lean.Json.toAdr (j : Json) : IO Adr := do
+  let x ← fromStr j >>= Hex.from0x
+  (Hex.toAdr x).toIO ""
+
+def Lean.Json.toB256? (j : Json) : IO B256 := do
+  let x ← fromStr j >>= Hex.from0x
+  (Hex.toB256? x).toIO ""
+
+def Lean.Json.toB256P (j : Json) : IO B256 := do
+  let x ← fromStr j >>= Hex.from0x
+  let xs ← (Hex.toB8L x).toIO ""
+  return (B8L.toB256P xs)
+
+def helper (xy :(_ : String) × Lean.Json) : IO (B256 × B256) := do
+  let x ← Hex.from0x xy.fst
+  let bs ← (Hex.toB8L x).toIO ""
+  let bs' ← xy.snd.toB8L
+  return ⟨bs.toB256P, bs'.toB256P⟩
+
+def Lean.Json.toPreData (sj : (_ : String) × Json) : IO PreData := do
+  let ax ← Hex.from0x sj.fst
+  let a ← (Hex.toAdr ax).toIO ""
+  let r ← sj.snd.fromObj
+  let b ← (r.find Ord.compare "balance").toIO "" >>= toB8L
+  let c ← (r.find Ord.compare "code").toIO "" >>= toB8L
+  let n ← (r.find Ord.compare "nonce").toIO "" >>= toB8L
+  let l ← (r.find Ord.compare "storage").toIO "" >>= fromObj
+  let s ← mapM helper l.toArray.toList
+  return ⟨a, n, b, Lean.RBMap.fromList s _, c⟩
+
+def Lean.Json.toEnvData (j : Lean.Json) : IO EnvData := do
+  let r ← j.fromObj
+  let bfj ← (r.find compare "currentBaseFee").toIO "No basefee"
+  let cbj ← (r.find compare "currentCoinbase").toIO "No coinbase"
+  let prj ← (r.find compare "currentRandom").toIO "No random"
+  let glj ← (r.find compare "currentGasLimit").toIO "No gas limit"
+  let tsj ← (r.find compare "currentTimestamp").toIO "No timestamp"
+  let nj  ← (r.find compare "currentNumber").toIO "No number"
+  let bf ← bfj.toB256P
+  let cb ← cbj.toAdr
+  let pr ← prj.toB256?
+  let gl ← glj.toB256P
+  let ts ← tsj.toB256P
+  let n  ← nj.toB256P
+  return {
+    baseFee := bf
+    coinbase := cb
+    prevRandao := pr
+    blockGasLimit := gl
+    timestamp := ts
+    number := n
+  }
+
+def Lean.Json.toPreDatas (j : Lean.Json) : IO (List PreData) := do
+  let r ← j.fromObj
+  let kvs := r.toArray.toList
+  mapM Lean.Json.toPreData kvs
+
+def Lean.Json.toPost (j : Lean.Json) : IO (String × List PostData) := do
+  let ⟨k, j'⟩ ← j.fromSingleton
+  let l ← j'.fromArr
+  let js ← mapM Lean.Json.toPostData l
+  return ⟨k, js⟩
+
+def Lean.Json.toTransactionData (j : Lean.Json) : IO TransactionData := do
+  let r ← j.fromObj
+  let ds ← (r.find Ord.compare "data").toIO "" >>= fromArr >>= mapM toB8L
+  let gls ← (r.find Ord.compare "gasLimit").toIO "" >>= fromArr >>= mapM toB256P
+  let gp ← ((r.find Ord.compare "gasPrice").toIO "" >>= toB256P)
+  let n ← ((r.find Ord.compare "nonce").toIO "" >>= toB256P)
+  let sk ← (r.find Ord.compare "secretKey").toIO "" >>= toB256?
+  let sd ← (r.find Ord.compare "sender").toIO "" >>= toAdr
+  let rc ← (r.find Ord.compare "to").toIO "" >>= toAdr
+  let vs ← (r.find Ord.compare "value").toIO "" >>= fromArr >>= mapM toB256P
+  return ⟨ds, gls, gp, n, sk, sd, rc, vs⟩
+
+def Lean.Json.toTestData (j : Lean.Json) : IO TestData := do
+  let (_, .obj r) ← j.fromSingleton | IO.throw "not singleton object"
+  let info ← (r.find compare "_info").toIO ""
+  let env ←  (r.find compare "env").toIO "" >>= Lean.Json.toEnvData
+  let pre ←  (r.find compare "pre").toIO "" >>= Lean.Json.toPreDatas
+  let post ← (r.find compare "post").toIO "" >>= Lean.Json.toPost
+  let tx ←   (r.find compare "transaction").toIO "" >>= Lean.Json.toTransactionData
+  return ⟨info, env, pre, post, tx⟩
+
+def TestData.world (td : TestData) : Option Wor :=
+  let aux : PreData → Option (Adr × Acct) :=
+    fun pd => do
+      some  ⟨
+        pd.addr,
+        {
+          nonce := pd.nonce.toB256P
+          bal := pd.bal.toB256P
+          stor := pd.stor
+          code := ByteArray.mk <| Array.mk pd.code
+        }
+    ⟩
+  do let l ← List.mapM aux td.pre
+     some <| Lean.RBMap.fromList l _
+
+def getTest (td : TestData) (p : PostData) : IO Test := do
+  let cd ← (List.get? td.tx.data p.dataIdx).toIO ""
+  let gl ← (List.get? td.tx.gasLimit p.gasIdx).toIO ""
+  let vl ← (List.get? td.tx.value p.valueIdx).toIO ""
+  let w ← td.world.toIO ""
+  return {
+    baseFee := td.env.baseFee
+    coinbase := td.env.coinbase
+    prevRandao := td.env.prevRandao
+    blockGasLimit := td.env.blockGasLimit
+    number := td.env.number
+    timestamp := td.env.timestamp
+    world := w
+    txdata := p.txdata
+    calldata := cd
+    gasLimit := gl
+    gasPrice := td.tx.gasPrice
+    nonce := td.tx.nonce
+    secret := td.tx.secretKey
+    sender := td.tx.sender
+    receiver := td.tx.receiver
+    value := vl
+    hash := p.hash
+    logs := p.logs
+  }
+
+def getTests (t : TestData) : IO (List Test) := do
+  have ps := t.post.snd
+  mapM (getTest t) ps
+
+def Lean.RBMap.fromSingleton {ξ υ f} (m : RBMap ξ υ f) : Option (ξ × υ) :=
+  match m.toList with
+  | [kv] => some kv
+  | _ => none
+
+def Lean.RBMap.singleton {ξ υ f} (x : ξ) (y : υ) : RBMap ξ υ f := RBMap.empty.insert x y
+
+inductive TxType : Type
+  | zero : TxType
+  -- access list (T_A)
+  | one : AccessList → TxType
+  -- access list (T_A), max fee per gas (T_m), max priority fee per gas (T_f)
+  | two : AccessList → B256 → B256 → TxType
+
+
+structure TxBytesContent : Type where
+  (chainId : Option Nat)
+  (yParity : Bool)
+  (type : TxType)
+  (nonce : B256)
+  (gasPrice : B256)
+  (gasLimit : B256)
+  (receiver : Adr)
+  (val : B256)
+  (calldata : B8L)
+  (r : B8L)
+  (s : B8L)
+  (acc : List (Adr × List B256))
+
+def decodeTxBytes (tbs : B8L) : IO (TxBytesContent × B256) :=
+  match RLP'.decode tbs with
+  | RLP'.list [
+      .b8s nonce,
+      .b8s gasPrice,
+      .b8s gasLimit,
+      .b8s receiver,
+      .b8s val,
+      .b8s calldata,
+      .b8s [v],
+      .b8s r,
+      .b8s s
+    ] => do
+    let bs :=
+      RLP'.encode <|
+        .list [
+          .b8s nonce,
+          .b8s gasPrice,
+          .b8s gasLimit,
+          .b8s receiver,
+          .b8s val,
+          .b8s calldata
+        ]
+    let recAdr ← (B8L.toAdr receiver).toIO "cannot convert bytes to receiver address"
+    return ⟨
+      {
+        chainId := none
+        yParity := if (v - 0x1B) = 0 then 0 else 1
+        type := .zero
+        nonce    := nonce.toB256P
+        gasPrice := gasPrice.toB256P
+        gasLimit := gasLimit.toB256P
+        receiver := recAdr
+        val := val.toB256P
+        calldata := calldata
+        r := (r.reverse.takeD 32 0).reverse
+        s := (s.reverse.takeD 32 0).reverse
+        acc := []
+      },
+      bs.keccak
+    ⟩
+  | _ => IO.throw "Error : TX bytes decoding failed"
